theory/bpfConsistencyAux.thy
@@ -44,6 +44,13 @@ fun exec_instrs :: "instruction list \<Rightarrow> outcome \<Rightarrow> outcome
   let st1 = exec_instr h 0 rs m in
     exec_instrs t st1
 )" 
+(*
+lemma hh1: assumes a0:" (xins, (Next reg m)) \<rightarrow>* ([], (Next reg'' m''))" and
+  a1:"length xins \<ge> (2::nat)"
+shows" \<exists> reg' m'. (xins, (Next reg m)) \<rightarrow>* (last xs, (Next reg' m')) \<and> (last xs, (Next reg' m')) \<rightarrow>* ([], (Next reg'' m''))  "
+  apply(induction "xins")
+   apply auto
+apply(rule small_steps.induct)*)
 
 (*
   BPF_DIV, BPF_MOD,  
@@ -99,48 +106,6 @@ lemma aluq_subgoal_rr_aux3:"op2 \<in> {BPF_SUB, BPF_MOV, BPF_ADD, BPF_AND, BPF_X
   apply(cases op2)
   apply(unfold eval_alu64_def,simp)
   by (unfold eval_alu64_aux1_def, simp_all)
-
-(*
-lemma addq_subgoal_rr:
-      "bins = BPF_ALU64 BPF_ADD dst (SOReg src) \<Longrightarrow>
-       xins = Paddq_rr rd ri \<Longrightarrow>
-       (BPF_OK pc rs' m' ss' is_v1 (cur_cu+1) remain_cu) = step fuel bins rs m ss is_v1 cur_cu remain_cu \<Longrightarrow>
-       Next reg' m' = exec_instr xins sz reg m \<Longrightarrow> 
-       rd = bpf_to_x64_reg dst \<Longrightarrow>
-       ri = bpf_to_x64_reg src \<Longrightarrow>
-       reg (IR rd) = Vlong n1 \<Longrightarrow>
-       reg (IR ri) = Vlong n2 \<Longrightarrow>
-       n1  = rs dst \<Longrightarrow>
-       n2  = rs src \<Longrightarrow>
-       Vlong (rs' dst) = reg' (IR (bpf_to_x64_reg dst))"
-  apply (unfold exec_instr_def step,simp_all)
-  apply (unfold eval_alu64_def)
-  apply (cases BPF_ADD, simp_all)
-  apply (unfold add64_def eval_alu64_aux1_def Let_def)
-  apply (cases BPF_ADD)
-  apply (unfold nextinstr_nf_def nextinstr_def eval_reg_def)
-  by simp_all
-
-lemma addq_subgoal_rr_aux2_1:"xins = Paddq_rr dst src \<Longrightarrow> Next reg' m' = exec_instr xins sz reg m \<Longrightarrow> \<forall> r \<noteq> dst . reg' (IR r) = reg (IR r)"
-  apply(unfold exec_instr_def, cases "xins", simp_all)
-  apply(unfold nextinstr_nf_def nextinstr_def add64_def) 
-  by auto
-
-lemma addq_subgoal_rr_aux2_2:"xins = Paddq_rr (bpf_to_x64_reg dst) (bpf_to_x64_reg src) \<Longrightarrow> Next reg' m' = exec_instr xins sz reg m \<Longrightarrow>
-       \<forall> r \<noteq> bpf_to_x64_reg dst. reg' (IR r) = reg (IR r)"
-  using addq_subgoal_rr_aux2_1 by blast
-
-lemma addq_subgoal_rr_aux2:"xins = Paddq_rr (bpf_to_x64_reg dst) (bpf_to_x64_reg src) \<Longrightarrow> Next reg' m' = exec_instr xins sz reg m \<Longrightarrow>
-       \<forall> r \<noteq> dst. reg' (IR (bpf_to_x64_reg r)) = reg (IR (bpf_to_x64_reg r))"
-  using bpf_to_x64_reg_corr addq_subgoal_rr_aux2_2 by metis
-
-lemma addq_subgoal_rr_aux3:"bins = BPF_ALU64 BPF_ADD dst (SOReg src) \<Longrightarrow> (BPF_OK pc rs' m' ss' is_v1 (cur_cu+1) remain_cu) = step fuel bins rs m ss is_v1 cur_cu remain_cu \<Longrightarrow>
-       \<forall> r \<noteq> dst. rs' r = rs r"
-  apply(cases "bins",simp_all)
-  apply(unfold eval_alu64_def,simp)
-  by (unfold eval_alu64_aux1_def, simp)
-
-*)
 
 subsubsection   \<open> BPF_ALU64 ADD64\<close>  
 
@@ -211,51 +176,6 @@ proof -
     have b7:"(\<forall> r \<noteq> dst. Vlong (rs' r) = reg' (IR (bpf_to_x64_reg r)))" by(simp add:b4 b5 b6) 
     thus ?thesis using b3 by fastforce
   qed
-
-(*
-lemma subq_subgoal_rr_aux1:
-     "bins = BPF_ALU64 BPF_SUB dst (SOReg src) \<Longrightarrow>
-     xins = Psubq_rr rd ri \<Longrightarrow>
-     (BPF_OK pc rs' m' ss' is_v1 (cur_cu+1) remain_cu) = step fuel bins rs m ss is_v1 cur_cu remain_cu \<Longrightarrow>
-     Next reg' m' = exec_instr xins sz reg m \<Longrightarrow>
-     rd = (bpf_to_x64_reg dst) \<Longrightarrow>
-     ri = (bpf_to_x64_reg src) \<Longrightarrow>
-     reg (IR rd) = Vlong n1 \<Longrightarrow>
-     reg (IR ri) = Vlong n2 \<Longrightarrow>
-     n1  = rs dst \<Longrightarrow>
-     n2  = rs src \<Longrightarrow> 
-     Vlong (rs' dst) = reg' (IR (bpf_to_x64_reg dst))"
-  apply (unfold exec_instr_def step)
-  apply simp
-  apply (unfold eval_alu64_def)
-  apply (cases BPF_SUB, simp_all)
-  apply (unfold eval_alu64_aux1_def)
-  apply (unfold Let_def)
-  apply (cases BPF_SUB, simp_all)
-  apply (unfold sub64_def)
-  apply (unfold nextinstr_nf_def nextinstr_def eval_reg_def)
-  by simp
-
-lemma subq_subgoal_rr_aux2_1:"xins = Psubq_rr dst src \<Longrightarrow> Next reg' m' = exec_instr xins sz reg m \<Longrightarrow> \<forall> r \<noteq> dst . reg' (IR r) = reg (IR r)"
-  apply(unfold exec_instr_def, cases "xins", simp_all)
-  apply(unfold nextinstr_nf_def nextinstr_def add64_def) 
-  by auto
-
-lemma subq_subgoal_rr_aux2_2:"xins = Psubq_rr (bpf_to_x64_reg dst) (bpf_to_x64_reg src) \<Longrightarrow> Next reg' m' = exec_instr xins sz reg m \<Longrightarrow>
-       \<forall> r \<noteq> bpf_to_x64_reg dst. reg' (IR r) = reg (IR r)"
-  using subq_subgoal_rr_aux2_1 by blast
-
-lemma subq_subgoal_rr_aux2:"xins = Psubq_rr (bpf_to_x64_reg dst) (bpf_to_x64_reg src) \<Longrightarrow> Next reg' m' = exec_instr xins sz reg m \<Longrightarrow>
-       \<forall> r \<noteq> dst. reg' (IR (bpf_to_x64_reg r)) = reg (IR (bpf_to_x64_reg r))"
-  using bpf_to_x64_reg_corr subq_subgoal_rr_aux2_2 by metis
-
-
-lemma subq_subgoal_rr_aux3:"bins = BPF_ALU64 BPF_SUB dst (SOReg src) \<Longrightarrow> (BPF_OK pc rs' m' ss' is_v1 (cur_cu+1) remain_cu) = step fuel bins rs m ss is_v1 cur_cu remain_cu \<Longrightarrow>
-       \<forall> r \<noteq> dst. rs' r = rs r"
-  apply(cases "bins",simp_all)
-  apply(unfold eval_alu64_def,simp)
-  by (unfold eval_alu64_aux1_def, simp)
-*)
 
 
 subsubsection   \<open> BPF_ALU64 MOV64\<close>
@@ -334,134 +254,9 @@ proof -
 lemma add_sub_consistency:"add64 (Vlong a) (Vlong b) = Vlong c \<Longrightarrow> sub64 (Vlong c) (Vlong a) = (Vlong b) "
   using add64_def sub64_def by auto
 
-(*lemma interp2_aux1:
-  assumes a0:"length xins = (2::nat)" and 
-          a1:"result = interp2 n xins (Next reg m)"
-        shows "result = Next reg' m' \<longrightarrow> n\<ge>2"
-proof (rule ccontr)
-  assume a2:"\<not> (result = Next reg' m' \<longrightarrow> n\<ge>2)"
-  let ?res_ok = "Next reg' m'"
-  have a3:"\<not> (\<not> result = ?res_ok \<or> (n\<ge>2))" using imp_conv_disj a2 by blast
-  have a4:"result = ?res_ok \<and> n<2" using a3 by simp
-   then show "False"
-   proof
-     have b0:"n<2" using a4 conjE by simp
-     have b2: "interp2 n xins (Next reg m) = Stuck"using a0 exec_instr_def 
-       by (smt (verit, del_insts) b0 interp2.elims interp2.simps(2) length_0_conv less_2_cases nat.inject outcome.simps(4) zero_neq_numeral)
-     thus "False" using b2 
-       using a1 a4 by (simp add: a0 exec_instr_def)
-   qed
- qed
-
-lemma interp2_aux2:
-  assumes a0:"length xins = (2::nat)" and 
-          a1:"result = interp2 n xins (Next reg m)"
-        shows "result = Next reg' m' \<longrightarrow> (exec_instr (xins!0) 1 reg m) \<noteq> Stuck"
-proof (rule ccontr)
-  assume a2:"\<not> (result = Next reg' m' \<longrightarrow> (exec_instr (xins!0) 1 reg m) \<noteq> Stuck)"
-  let ?tmp = "(exec_instr (xins!0) 1 reg m) "
-  let ?res_ok = "Next reg' m'"
-  have a3:"\<not> (\<not> result = ?res_ok \<or> ?tmp \<noteq> Stuck)" using imp_conv_disj a2 by blast
-  have a4:"result = ?res_ok \<and> ?tmp = Stuck" using a3 by simp
-   then show "False"
-   proof
-     have b0:"?tmp = Stuck" using a4 conjE by simp
-     have b1:"xins\<noteq>[]" using a0 by auto
-     have b2: "interp2 n xins (Next reg m) = Stuck"using a0 b0 b1 exec_instr_def 
-       by (smt (verit, del_insts) interp2.elims nth_Cons_0 outcome.case(2) outcome.simps(4))
-     thus "False" using b2 
-       using a1 a4 by (simp add: a0 exec_instr_def)
-   qed
- qed
-
-(*interp2 n (drop 1 xins) (Next reg' m') = (exec_instr (xins!1) 1 reg' m')*)
-lemma interp2_aux3:
-  assumes a0:"length xins = (2::nat)" and 
-          a1:"result = interp2 n xins (Next reg m)" and
-          a2:"Next reg' m' = (exec_instr (xins!0) 1 reg m)"
-        shows "result = Next reg'' m'' \<longrightarrow> (exec_instr (xins!1) 1 reg' m') \<noteq> Stuck"
-proof (rule ccontr)
-  assume a2:"\<not> (result = Next reg'' m'' \<longrightarrow> (exec_instr (xins!1) 1 reg' m') \<noteq> Stuck)"
-  let ?tmp = "(exec_instr (xins!1) 1 reg' m') "
-  let ?res_ok = "Next reg'' m''"
-  have a3:"\<not> (\<not> result = ?res_ok \<or> ?tmp \<noteq> Stuck)" using imp_conv_disj a2 by blast
-  have a4:"result = ?res_ok \<and> ?tmp = Stuck" using a3 by simp
-   then show "False"
-   proof
-     have b0:"?tmp = Stuck" using a4 conjE by simp
-     have b1:"xins\<noteq>[]" using a0 by auto
-     have b2:"interp2 (n-1) (drop 1 xins) (Next reg' m') = (exec_instr (xins!1) 1 reg' m')" using a0 a1 a2 b1 
-       by (smt (verit, ccfv_threshold) Cons_nth_drop_Suc One_nat_def Suc_n_not_le_n drop_eq_Nil interp2.elims lessI list.inject numeral_2_eq_2 outcome.case(2) outcome.simps(4))
-     have b3: "interp2 (n-1) (drop 1 xins) (Next reg' m') = Stuck"using a0 b0 b1 exec_instr_def a2
-       using interp2.elims nth_Cons_0 outcome.case(2) outcome.simps(4) using b2 by simp
-     have b4: "interp2 n xins (Next reg m) = Stuck" using a0 a1 b3 exec_instr_def a2 b1
-       by (smt (verit) Cons_nth_drop_Suc One_nat_def Suc_n_not_le_n assms(3) drop0 drop_eq_Nil interp2.elims list.inject list_consists_2 numeral_2_eq_2 outcome.case(2) outcome.simps(4) zero_less_Suc)
-     thus "False" using b2 
-       using a1 a4 by (simp add: a0 exec_instr_def)
-   qed
- qed
-
-
-lemma interp2_aux4:"n > 0 \<Longrightarrow> interp2 n [] (Next reg m) = Next reg m"
-  by (metis Suc_pred interp2.simps(2))
-
-
-lemma interp2_aux4: assumes a0:"Next reg2 m2 = interp2 n xins (Next reg m)" and
-  a1:"length xins = (2::nat)"
-shows" \<exists> reg' m'. Next reg' m' = (exec_instr (xins!0) 1 reg m) \<and> Next reg2 m2 = (exec_instr (xins!1) 1 reg' m')  "
-proof-
-  have b0:"n\<ge>2" using a0 a1 interp2_aux1 by blast
-  from a0 a1 have "\<exists> result1. result1 = (exec_instr (xins!0) 1 reg m)" by simp
-  then obtain result1 where " result1 = (exec_instr (xins!0) 1 reg m)" by simp
-  have b1:"result1 \<noteq> Stuck" using interp2_aux2 a0 a1 
-    by (metis \<open>(result1::outcome) = exec_instr ((xins::instruction list) ! (0::nat)) (1::64 word) (reg::preg \<Rightarrow> val) (m::64 word \<Rightarrow> 8 word option option)\<close> a0 a1)
-  from b1 have "\<exists> reg' m'. Next reg' m' = result1" 
-    by (metis outcome.exhaust)
-  then obtain reg' m' where "Next reg' m' = result1" by blast
-  have "\<exists> result2. result2 = (exec_instr (xins!1) 1 reg' m')" by simp
-  then obtain result2 where " result2 = (exec_instr (xins!1) 1 reg' m')" by simp
-  have b3:"result2 \<noteq> Stuck" using interp2_aux3 a0 a1 
-    by (metis \<open>(result1::outcome) = exec_instr ((xins::instruction list) ! (0::nat)) (1::64 word) (reg::preg \<Rightarrow> val) (m::64 word \<Rightarrow> 8 word option option)\<close> \<open>(result2::outcome) = exec_instr ((xins::instruction list) ! (1::nat)) (1::64 word) (reg'::preg \<Rightarrow> val) (m'::64 word \<Rightarrow> 8 word option option)\<close> \<open>Next (reg'::preg \<Rightarrow> val) (m'::64 word \<Rightarrow> 8 word option option) = (result1::outcome)\<close>)
-  then obtain reg'' m'' where "Next reg'' m'' = result2" 
-    by (metis outcome.exhaust)
-  have b4:"Next reg'' m'' = Next reg2 m2" using b1 interp2_aux4 interp2_aux1 try
-  show ?thesis using a0 a1 b0 
-    using \<open>(result1::outcome) = exec_instr ((xins::instruction list) ! (0::nat)) (1::64 word) (reg::preg \<Rightarrow> val) (m::64 word \<Rightarrow> 8 word option option)\<close> \<open>(result2::outcome) = exec_instr ((xins::instruction list) ! (1::nat)) (1::64 word) (reg'::preg \<Rightarrow> val) (m'::64 word \<Rightarrow> 8 word option option)\<close> \<open>Next (reg''::preg \<Rightarrow> val) (m''::64 word \<Rightarrow> 8 word option option) = (result2::outcome)\<close> \<open>Next (reg'::preg \<Rightarrow> val) (m'::64 word \<Rightarrow> 8 word option option) = (result1::outcome)\<close> b4 by blast
-qed
-lemma shift_subgoal_rr_aux1_1:"Next reg'' m'' = interp2 n xins (Next reg m) \<Longrightarrow> length xins = (2::nat) \<Longrightarrow> \<exists> reg' m'. Next reg' m' = (exec_instr (xins!0) 1 reg m) \<and> Next reg'' m'' = (exec_instr (xins!1) 1 reg' m')  "
-  using interp2_aux4 by simp
-
-
-lemma shift_subgoal_rr_aux1_2:
-  assumes a0:"length xins = (2::nat)" and a1:"Next reg' m' = (exec_instr (xins!0) 1 reg m)" and a1:" Next reg'' m'' = (exec_instr (xins!1) 1 reg' m')"
-  shows "Next reg'' m'' = interp2 n xins (Next reg m)"
-  sorry
-
-lemma shift_subgoal_rr_aux2:
-  assumes a0:"xins = [(Pmovq_rr src (x64Syntax.RCX)),(Pshlq_r dst)]" and 
-    a1:"Next reg'' m'' = interp2 n xins (Next reg m) " 
-  shows " m'' = m"
-proof-
-  have b0:"length xins = (2::nat)" using a0 by simp
-  thus ?thesis using b0 a0 a1 shift_subgoal_rr_aux2_3 
-    by (meson shift_subgoal_rr_aux1_1)
-qed
-
-
-lemma push_pop_subgoal_rr_aux2_2:
-  assumes a0:"xins = [Ppushl_r x64Syntax.RCX, Ppopl x64Syntax.RCX]" and 
-    a1:"Next reg'' m'' = interp2 n xins (Next reg m)" and
-    a2:"storev M32 m (sub64 (reg (IR SP)) (vlong_of_memory_chunk M32)) (reg (IR ireg.RCX)) \<noteq> None "
-  shows "reg'' (IR x64Syntax.RCX) = reg (IR x64Syntax.RCX)"
-proof-
-  have b0:"length xins = (2::nat)" using a0 by simp
-  thus ?thesis using b0 a0 a1 a2 push_pop_subgoal_rr_aux2_1 shift_subgoal_rr_aux1_1
-    by metis
-qed
-*)
 
 lemma interp3_aux2:
-  assumes a0:"length xins = (2::nat)" and 
+  assumes a0:"xins\<noteq>[]" and 
           a1:"result = interp3 xins (Next reg m)"
         shows "result = Next reg' m' \<longrightarrow> (exec_instr (xins!0) 1 reg m) \<noteq> Stuck"
 proof (rule ccontr)
@@ -473,8 +268,7 @@ proof (rule ccontr)
    then show "False"
    proof
      have b0:"?tmp = Stuck" using a4 conjE by simp
-     have b1:"xins\<noteq>[]" using a0 by auto
-     have b2: "interp3 xins (Next reg m) = Stuck"using a0 b0 b1 exec_instr_def 
+     have b2: "interp3 xins (Next reg m) = Stuck"using a0 b0 exec_instr_def 
        by (smt (verit, del_insts) interp3.elims nth_Cons_0 outcome.case(2) outcome.simps(4))
      thus "False" using b2 
        using a1 a4 by (simp add: a0 exec_instr_def)
@@ -508,6 +302,34 @@ proof (rule ccontr)
    qed
  qed
 
+lemma interp3_length4_aux1:
+  assumes a0:"xins\<noteq>[]" and 
+          a1:"result = interp3 xins (Next reg m)" and
+          a2:"Next reg' m' = (exec_instr (xins!0) 1 reg m)"
+        shows "result = Next reg'' m'' \<longrightarrow> interp3 (tl xins) (Next reg' m') \<noteq> Stuck"
+proof (rule ccontr)
+  assume a2:"\<not> (result = Next reg'' m'' \<longrightarrow> interp3 (tl xins) (Next reg' m') \<noteq> Stuck)"
+  let ?tmp = "interp3 (tl xins) (Next reg' m') "
+  let ?res_ok = "Next reg'' m''"
+  have a3:"\<not> (\<not> result = ?res_ok \<or> ?tmp \<noteq> Stuck)" using imp_conv_disj a2 by blast
+  have a4:"result = ?res_ok \<and> ?tmp = Stuck" using a3 by simp
+   then show "False"
+   proof
+     have b0:"?tmp = Stuck" using a4 conjE by simp
+     have b1:"xins\<noteq>[]" using a0 by auto
+     have b2:"interp3 (tl xins) (Next reg' m') = interp3 (xins) (Next reg m)" using a0 a1 a2 b0 b1 
+       by (metis assms(3) hd_conv_nth interp3.simps(2) list.exhaust list.sel(1) list.sel(3) outcome.simps(4))
+     have b3: "interp3 (tl xins) (Next reg' m') = Stuck"using a0 b0 b1 exec_instr_def a2
+       using interp2.elims nth_Cons_0 outcome.case(2) outcome.simps(4) using b2 by simp
+     have b4: "interp3 xins (Next reg m) = Stuck" using a0 a1 b3 exec_instr_def a2 
+       using b2 by argo
+     thus "False" using b2 
+       using a1 a4 by (simp add: a0 exec_instr_def)
+   qed
+ qed
+
+
+
 lemma interp3_aux4:"interp3 [] (Next reg m) = Next reg m"
   by simp
 
@@ -517,7 +339,8 @@ shows" \<exists> reg' m'. Next reg' m' = (exec_instr (xins!0) 1 reg m) \<and> Ne
 proof-
   from a0 a1 have "\<exists> result1. result1 = (exec_instr (xins!0) 1 reg m)" by simp
   then obtain result1 where " result1 = (exec_instr (xins!0) 1 reg m)" by simp
-  have b1:"result1 \<noteq> Stuck" using interp3_aux2 a0 a1 
+  have b1_1:"xins\<noteq>[]" using a1 by auto
+  have b1:"result1 \<noteq> Stuck" using interp3_aux2 a0 b1_1 
     by (metis \<open>(result1::outcome) = exec_instr ((xins::instruction list) ! (0::nat)) (1::64 word) (reg::preg \<Rightarrow> val) (m::64 word \<Rightarrow> 8 word option option)\<close> a0 a1)
   from b1 have "\<exists> reg' m'. Next reg' m' = result1" 
     by (metis outcome.exhaust)
@@ -533,6 +356,222 @@ proof-
   show ?thesis using a0 a1 
     using \<open>(result1::outcome) = exec_instr ((xins::instruction list) ! (0::nat)) (1::64 word) (reg::preg \<Rightarrow> val) (m::64 word \<Rightarrow> 8 word option option)\<close> \<open>(result2::outcome) = exec_instr ((xins::instruction list) ! (1::nat)) (1::64 word) (reg'::preg \<Rightarrow> val) (m'::64 word \<Rightarrow> 8 word option option)\<close> \<open>Next (reg''::preg \<Rightarrow> val) (m''::64 word \<Rightarrow> 8 word option option) = (result2::outcome)\<close> \<open>Next (reg'::preg \<Rightarrow> val) (m'::64 word \<Rightarrow> 8 word option option) = (result1::outcome)\<close> b4 by blast
 qed
+
+lemma interp3_length4_aux2:
+  assumes a0:"length xins = (4::nat)" and 
+          a1:"result = interp3 xins (Next reg m)" and
+          a2:"Next reg2 m2 = interp3 (take 2 xins) (Next reg m)"
+        shows "result = Next reg'' m'' \<longrightarrow> interp3 (drop 2 xins) (Next reg2 m2) \<noteq> Stuck"
+proof (rule ccontr)
+  assume a2:"\<not> (result = Next reg'' m'' \<longrightarrow> interp3 (drop 2 xins) (Next reg2 m2) \<noteq> Stuck)"
+  let ?tmp = "interp3 (drop 2 xins) (Next reg2 m2) "
+  let ?res_ok = "Next reg'' m''"
+  have a3:"\<not> (\<not> result = ?res_ok \<or> ?tmp \<noteq> Stuck)" using imp_conv_disj a2 by blast
+  have a4:"result = ?res_ok \<and> ?tmp = Stuck" using a3 by simp
+   then show "False"
+   proof
+     have b0:"?tmp = Stuck" using a4 conjE by simp
+     have b1:"(take 2 xins) @ (drop 2 xins)= xins" using a0
+       by (simp add: Cons_nth_drop_Suc numeral_3_eq_3 numeral_nat(2))
+     let ?tmplist = "take 2 xins"
+     have b2_1:"?tmplist = [(xins!0)]@[(xins!1)]" 
+       by (metis One_nat_def Suc_1 a0 append_Nil less_1_mult less_2_cases_iff numeral_Bit0_eq_double take_0 take_Suc_conv_app_nth zero_less_numeral)
+     have b2_2:"length ?tmplist = (2::nat)" 
+       by (simp add: b2_1)
+     have b2_3:"\<exists> reg1 m1. Next reg1 m1 = (exec_instr (xins!0) 1 reg m) \<and> Next reg2 m2 = (exec_instr (xins!1) 1 reg1 m1 )" using a2 b2_2 b2_1 interp3_aux5 
+       by (metis Cons_eq_appendI One_nat_def append_Nil assms(3) nth_Cons_0 nth_Cons_Suc)
+     then obtain reg1 m1 where b2_4:"Next reg1 m1 = (exec_instr (xins!0) 1 reg m) \<and> Next reg2 m2 = (exec_instr (xins!1) 1 reg1 m1 )" by auto
+     have b2_5:"Next reg1 m1 = (exec_instr (xins!0) 1 reg m)" using b2_3 using b2_4 by blast
+     have b2_6:" Next reg2 m2 = (exec_instr (xins!1) 1 reg1 m1 )" using b2_3 using b2_4 by blast
+     have b2_7:"[xins!0]@[xins!1] @ (drop 2 xins)= xins" using a0
+       by (simp add: Cons_nth_drop_Suc numeral_3_eq_3 numeral_nat(2))
+     have b2:"interp3 (drop 2 xins) (Next reg2 m2) = interp3 (xins) (Next reg m)" using a0 a1 a2 a3 b0 
+       using append_Cons append_Nil assms(3) b2_5 b2_6 b2_7 interp3.simps(2) outcome.simps(4) by metis
+     have b3: "interp3 (drop 2 xins) (Next reg2 m2) = Stuck"using a0 b0 b1 exec_instr_def a2
+       using interp2.elims nth_Cons_0 outcome.case(2) outcome.simps(4) by auto
+     have b4: "interp3 xins (Next reg m) = Stuck" using a0 a1 b3 exec_instr_def a2 
+       using b2 by argo
+     thus "False" using b2 
+       using a1 a4 by (simp add: a0 exec_instr_def)
+   qed
+ qed
+
+(*
+lemma interp3_length4_aux2:
+  assumes a0:"length xins = (4::nat)" and 
+          a1:"result = interp3 xins (Next reg m)" and
+          a2:"Next reg1 m1 = (exec_instr (xins!0) 1 reg m)" and
+          a3:"Next reg2 m2 = (exec_instr (xins!1) 1 reg1 m1)" (*"Next reg' m' = interp3 (take 2 xins) (Next reg m)"*)
+        shows "result = Next reg'' m'' \<longrightarrow> interp3 (drop 2 xins) (Next reg2 m2) \<noteq> Stuck"
+proof (rule ccontr)
+  assume a2:"\<not> (result = Next reg'' m'' \<longrightarrow> interp3 (drop 2 xins) (Next reg2 m2) \<noteq> Stuck)"
+  let ?tmp = "interp3 (drop 2 xins) (Next reg2 m2) "
+  let ?res_ok = "Next reg'' m''"
+  have a3:"\<not> (\<not> result = ?res_ok \<or> ?tmp \<noteq> Stuck)" using imp_conv_disj a2 by blast
+  have a4:"result = ?res_ok \<and> ?tmp = Stuck" using a3 by simp
+   then show "False"
+   proof
+     have b0:"?tmp = Stuck" using a4 conjE by simp
+     have b1:"[xins!0]@[xins!1] @ (drop 2 xins)= xins" using a0
+       by (simp add: Cons_nth_drop_Suc numeral_3_eq_3 numeral_nat(2))
+     have b2:"interp3 (drop 2 xins) (Next reg2 m2) = interp3 (xins) (Next reg m)" using a0 a1 a2 a3 b0 b1 
+       by (metis append_Cons append_Nil assms(3) assms(4) interp3.simps(2) outcome.simps(4))
+     have b3: "interp3 (drop 2 xins) (Next reg2 m2) = Stuck"using a0 b0 b1 exec_instr_def a2
+       using interp2.elims nth_Cons_0 outcome.case(2) outcome.simps(4) using b2 by simp
+     have b4: "interp3 xins (Next reg m) = Stuck" using a0 a1 b3 exec_instr_def a2 
+       using b2 by argo
+     thus "False" using b2 
+       using a1 a4 by (simp add: a0 exec_instr_def)
+   qed
+ qed
+*)
+
+lemma interp3_length4_aux3:
+  assumes a0:"length xins = (4::nat)" and 
+          a1:"result = interp3 xins (Next reg m)" and
+          a2:"Next reg1 m1 = (exec_instr (xins!0) 1 reg m)" and
+          a3:"Next reg2 m2 = (exec_instr (xins!1) 1 reg1 m1)" and
+          a4:"Next reg' m' = (exec_instr (xins!2) 1 reg2 m2)"  (*"Next reg' m' = interp3 (butlast xins) (Next reg m)"*)
+        shows "result = Next reg'' m'' \<longrightarrow> (exec_instr (xins!3) 1 reg' m') \<noteq> Stuck"
+proof (rule ccontr)
+  assume a2:"\<not> (result = Next reg'' m'' \<longrightarrow> (exec_instr (xins!3) 1 reg' m') \<noteq> Stuck)"
+  let ?tmp = "(exec_instr (xins!3) 1 reg' m') "
+  let ?res_ok = "Next reg'' m''"
+  have a3:"\<not> (\<not> result = ?res_ok \<or> ?tmp \<noteq> Stuck)" using imp_conv_disj a2 by blast
+  have a4:"result = ?res_ok \<and> ?tmp = Stuck" using a3 by simp
+   then show "False"
+   proof
+     have b0:"?tmp = Stuck" using a4 conjE by simp
+     have b1:"[(xins!0)]@[(xins!1)]@[(xins!2)]@[(xins!3)] = xins"
+       using a0 
+       by (metis Cons_eq_appendI One_nat_def append_Nil last.simps list.discI list_consists_4)
+     have b2:"exec_instr (xins!3) 1 reg' m' = interp3 (xins) (Next reg m)" using a0 a1 a2 a3 a4 b0 b1 
+       by (metis Cons_eq_appendI append_Nil assms(3) assms(4) assms(5) interp3.simps(1) interp3.simps(2) interp3_length4_aux1 list.sel(3) outcome.simps(4))
+     have b4: "interp3 xins (Next reg m) = Stuck" using a0 a1 b2 exec_instr_def a2 
+       by simp
+     thus "False" using b2 
+       using a1 a4 by (simp add: a0 exec_instr_def)
+   qed
+ qed
+
+lemma interp3_aux6:
+  assumes a0:"length xins > i" and 
+          a1:"result = interp3 xins (Next reg m)" and
+          a2:"Next reg' m' = interp3 (take i xins) (Next reg m)"
+        shows "result = Next reg'' m'' \<longrightarrow> (exec_instr (xins!(i+1)) 1 reg' m') \<noteq> Stuck"
+proof (rule ccontr)
+  assume a2:"\<not> (result = Next reg'' m'' \<longrightarrow> (exec_instr (xins!(i+1)) 1 reg' m') \<noteq> Stuck)"
+  let ?tmp = "(exec_instr (xins!(i+1)) 1 reg' m') "
+  let ?res_ok = "Next reg'' m''"
+  have a3:"\<not> (\<not> result = ?res_ok \<or> ?tmp \<noteq> Stuck)" using imp_conv_disj a2 by blast
+  have a4:"result = ?res_ok \<and> ?tmp = Stuck" using a3 by simp
+   then show "False"
+   proof
+     have b0:"?tmp = Stuck" using a4 conjE by simp
+     have b1:"length xins - i > 0" using a0 by auto
+     have b2:"interp3 [xins!(i+1)] (Next reg' m') = (exec_instr (xins!(i+1)) 1 reg' m')" using a0 a1 a2 b0 b1 
+       by (metis Cons_nth_drop_Suc Suc_eq_plus1 drop_eq_Nil interp3.simps(1) interp3.simps(2) le_refl lessI nat_1_add_1 outcome.simps(4))
+     have b3: "interp3 [xins!(i+1)] (Next reg' m') = Stuck"using a0 b0 b1 exec_instr_def a2
+       using interp2.elims nth_Cons_0 outcome.case(2) outcome.simps(4) using b2 by simp
+     have b4: "interp3 (take (i+1) xins) (Next reg m) = Stuck" using a0 a1 b3 exec_instr_def a2 
+       sorry
+     have b5: "interp3 xins (Next reg m) = Stuck" using b4 sorry
+     thus "False" using b2 
+       using a1 a4 by (simp add: a0 exec_instr_def)
+   qed
+ qed
+
+lemma interp3_aux7: assumes a0:"Next reg2 m2 = interp3 xins (Next reg m)" and
+  a1:"length xins = (4::nat)"
+shows" \<exists> reg' m'. Next reg' m' = (exec_instr (xins!0) 1 reg m) \<and> Next reg2 m2 = (exec_instr (xins!1) 1 reg' m')  "
+proof-
+  from a0 a1 have "\<exists> result1. result1 = (exec_instr (xins!0) 1 reg m)" by simp
+  then obtain result1 where " result1 = (exec_instr (xins!0) 1 reg m)" by simp
+  have b1_1:"xins\<noteq>[]" using a1 by auto
+  have b1:"result1 \<noteq> Stuck" using interp3_aux2 a0 b1_1 
+    by (metis \<open>(result1::outcome) = exec_instr ((xins::instruction list) ! (0::nat)) (1::64 word) (reg::preg \<Rightarrow> val) (m::64 word \<Rightarrow> 8 word option option)\<close> a0 a1)
+  from b1 have "\<exists> reg' m'. Next reg' m' = result1" 
+    by (metis outcome.exhaust)
+  then obtain reg' m' where "Next reg' m' = result1" by blast
+  have "\<exists> result2. result2 = (exec_instr (xins!1) 1 reg' m')" by simp
+  then obtain result2 where " result2 = (exec_instr (xins!1) 1 reg' m')" by simp
+  have b3:"result2 \<noteq> Stuck" using interp3_aux3 a0 a1 
+    by (metis \<open>(result1::outcome) = exec_instr ((xins::instruction list) ! (0::nat)) (1::64 word) (reg::preg \<Rightarrow> val) (m::64 word \<Rightarrow> 8 word option option)\<close> \<open>(result2::outcome) = exec_instr ((xins::instruction list) ! (1::nat)) (1::64 word) (reg'::preg \<Rightarrow> val) (m'::64 word \<Rightarrow> 8 word option option)\<close> \<open>Next (reg'::preg \<Rightarrow> val) (m'::64 word \<Rightarrow> 8 word option option) = (result1::outcome)\<close>)
+  then obtain reg'' m'' where "Next reg'' m'' = result2" 
+    by (metis outcome.exhaust)
+  have b4:"Next reg'' m'' = Next reg2 m2" using interp3_aux4 a1 
+    by (metis Suc_eq_plus1 \<open>(result1::outcome) = exec_instr ((xins::instruction list) ! (0::nat)) (1::64 word) (reg::preg \<Rightarrow> val) (m::64 word \<Rightarrow> 8 word option option)\<close> \<open>(result2::outcome) = exec_instr ((xins::instruction list) ! (1::nat)) (1::64 word) (reg'::preg \<Rightarrow> val) (m'::64 word \<Rightarrow> 8 word option option)\<close> \<open>Next (reg''::preg \<Rightarrow> val) (m''::64 word \<Rightarrow> 8 word option option) = (result2::outcome)\<close> \<open>Next (reg'::preg \<Rightarrow> val) (m'::64 word \<Rightarrow> 8 word option option) = (result1::outcome)\<close> a0 add.commute add.right_neutral interp3.simps(2) list_consists_2 outcome.simps(4))
+  show ?thesis using a0 a1 
+    using \<open>(result1::outcome) = exec_instr ((xins::instruction list) ! (0::nat)) (1::64 word) (reg::preg \<Rightarrow> val) (m::64 word \<Rightarrow> 8 word option option)\<close> \<open>(result2::outcome) = exec_instr ((xins::instruction list) ! (1::nat)) (1::64 word) (reg'::preg \<Rightarrow> val) (m'::64 word \<Rightarrow> 8 word option option)\<close> \<open>Next (reg''::preg \<Rightarrow> val) (m''::64 word \<Rightarrow> 8 word option option) = (result2::outcome)\<close> \<open>Next (reg'::preg \<Rightarrow> val) (m'::64 word \<Rightarrow> 8 word option option) = (result1::outcome)\<close> b4 by blast
+qed
+
+
+lemma run_trans: "\<forall> A B C as bs. interp3 as A  = B \<and> interp3 bs B = C \<longrightarrow> interp3 (as @ bs) A = C"
+  proof-
+  {
+    fix B C as bs
+    have "\<forall> A. interp3 as A  = B \<and> interp3 bs B = C \<longrightarrow> interp3 (as @ bs) A = C"
+      proof(induct as)
+        case Nil then show ?case by simp
+      next
+        case (Cons c cs)
+        assume a0: "\<forall>A. interp3 cs A = B \<and> interp3 bs B = C \<longrightarrow> interp3 (cs @ bs) A = C"
+        show ?case
+          proof-
+            fix A
+            have "interp3 (c # cs) A  = B \<and> interp3 bs B = C \<longrightarrow> interp3 ((c # cs) @ bs) A = C"
+            proof
+              assume b0: "interp3 (c # cs) A = B \<and> interp3 bs B = C"
+
+              from b0 obtain A' where b2: "interp3 [c] A  = A' \<and> interp3 cs A' = B" 
+              proof(cases A)
+                case (Next x11 x12)
+                then show ?thesis sorry
+              next
+                case Stuck
+                then show ?thesis sorry
+              qed
+              with a0 b0 have "interp3 (cs @ bs) A' = C"
+                using local.Cons by blast
+              with b2 show "interp3 ((c # cs) @ bs) A = C" 
+                by simp
+            qed
+          then show ?thesis using a0 by auto
+          qed
+      qed
+  }
+  then show ?thesis by auto
+  qed
+
+
+lemma run_trans: "\<forall> A B C as bs. interp4 as A  = B \<and> interp4 bs B = C \<longrightarrow> interp4 (as @ bs) A = C"
+  proof-
+  {
+    fix B C as bs
+    have "\<forall> A. interp4 as A  = B \<and> interp4 bs B = C \<longrightarrow> interp4 (as @ bs) A = C"
+      proof(induct as)
+        case Nil then show ?case by simp
+      next
+        case (Cons c cs)
+        assume a0: "\<forall>A. interp4 cs A = B \<and> interp4 bs B = C \<longrightarrow> interp4 (cs @ bs) A = C"
+        show ?case
+          proof-
+            fix A
+            have "interp4 (c # cs) A  = B \<and> interp4 bs B = C \<longrightarrow> interp4 ((c # cs) @ bs) A = C"
+            proof
+              assume b0: "interp4 (c # cs) A = B \<and> interp4 bs B = C"
+              from b0 obtain A' where b2: "interp4 [c] A  = A' \<and> interp4 cs A' = B" by simp
+              with a0 b0 have "interp4 (cs @ bs) A' = C"
+                using local.Cons by blast
+              with b2 show "interp4 ((c # cs) @ bs) A = C" 
+                by simp
+            qed
+          then show ?thesis using a0 by auto
+          qed
+      qed
+  }
+  then show ?thesis by auto
+  qed
 
 lemma shift_subgoal_rr_aux1_1:"Next reg'' m'' = interp3 xins (Next reg m) \<Longrightarrow> length xins = (2::nat) \<Longrightarrow> \<exists> reg' m'. Next reg' m' = (exec_instr (xins!0) 1 reg m) \<and> Next reg'' m'' = (exec_instr (xins!1) 1 reg' m')  "
   using interp3_aux5 by simp
@@ -719,6 +758,28 @@ proof-
   thus ?thesis using c4 by simp
 qed
 
+lemma hh1: assumes a0:"Next reg'' m'' = interp3 xins (Next reg m)" and
+  a1:"length xins \<ge> (2::nat)"
+shows" \<exists> reg' m'. Next reg' m' = interp3 (butlast xins) (Next reg m) \<and> Next reg'' m'' = (exec_instr (last xins) 1 reg' m')   "
+  sorry
+
+
+(*lemma hh2: assumes a0:"Next reg'' m'' = interp3 xins (Next reg m)" and
+  a1:"length xins \<ge> (2::nat)" and
+  a2:"length xins \<ge> (2::nat)"
+shows" \<exists> reg' m'. Next reg' m' = interp3 (butlast xins) (Next reg m) \<and> Next reg'' m'' = (exec_instr (last xins) 1 reg' m')   "
+  sorry
+*)
+
+
+lemma hh2:
+  assumes a0:"xins = [Ppushl_r x64Syntax.RCX, Pmovq_rr (x64Syntax.RCX) (bpf_to_x64_reg src),Pshlq_r (bpf_to_x64_reg dst),Ppopl x64Syntax.RCX]" and 
+    a1:"Next reg'' m'' = interp3 xins (Next reg m)" and
+    a2:"Next reg' m' = (exec_instr (xins!0) 1 reg m)"
+  shows "\<exists> reg2 m2. interp3 (butlast(tl xins)) (Next reg' m') = Next reg2 m2"
+  sorry
+
+
 
 lemma shift_subgoal_rr_aux4_1:
   assumes a0:"xins = [Ppushl_r x64Syntax.RCX, Pmovq_rr (x64Syntax.RCX) (bpf_to_x64_reg src),Pshlq_r (bpf_to_x64_reg dst),Ppopl x64Syntax.RCX]" and 
@@ -733,16 +794,21 @@ proof-
     using a1 exec_push_def a0 
     by (smt (verit, del_insts) instruction.simps(6295) interp3.simps(2) option.case_eq_if outcome.case(2) outcome.simps(4))
   then obtain reg' m' where b0:"Next reg' m' = exec_push 1 M32 m reg (reg (IR x64Syntax.RCX))" by blast
-  have b2:"\<exists> reg2 m2. interp3 ?midlist (Next reg' m') = Next reg2 m2" sorry
+  have b2:"\<exists> reg2 m2. interp3 ?midlist (Next reg' m') = Next reg2 m2" using hh2 b1 a0 a1 
+    by (smt (verit) One_nat_def Suc_eq_plus1 Suc_leI Suc_le_mono b0 butlast.simps(2) exec_instr_def hh1 instruction.case(60) interp3.elims interp3.simps(2) list.distinct(1) list.sel(1) list.size(3) list.size(4) nat_1_add_1 nth_Cons_0 numeral_2_eq_2 outcome.simps(4) zero_less_Suc)
   then obtain reg2 m2 where b3:"interp3 ?midlist (Next reg' m') = Next reg2 m2" by auto
   have b4:"m2 = m'" using shift_subgoal_rr_aux2 by (metis b3)
   have b5:"reg' (IR SP) =  reg2 (IR SP)" using shift_subgoal_rr_aux3 b3 by metis
   have b6:"Next reg' m' = (exec_instr (xins!0) 1 reg m) " using a0 by (simp add: b0 exec_instr_def)
-  have b7:"Next reg'' m'' = (exec_instr (last xins) 1 reg2 m2)" sorry
+  have b7_1:"length xins \<ge> (2::nat)" using a0 by simp
+  have b7_2:"Next reg2 m2 = interp3 (butlast xins) (Next reg m)" using b3 b0 a0 by (simp add: b6)
+  have b7:"Next reg'' m'' = (exec_instr (last xins) 1 reg2 m2)" using hh1 b7_1 b7_2 by (metis a1 outcome.inject)
   have b8:"Next reg'' m'' = (exec_instr (last xins) 1 reg2 m')" using b7 b4 by simp
   thus ?thesis using a3 a4 b4 b5 b6 b8 a1 push_pop_subgoal_rr_aux2_3
     by (metis a0 b3 butlast.simps(2) list.distinct(1) list.sel(3))
 qed
+
+
 
 lemma shift_subgoal_rr_aux4_2:"xins = Pmovq_rr (x64Syntax.RCX) src \<Longrightarrow> 
     Next reg' m' = (exec_instr xins 1 reg m)\<Longrightarrow> 
@@ -792,7 +858,7 @@ proof-
   thus ?thesis using b2 by simp
 qed
 
-lemma shift_subgoal_rr_aux5:
+lemma shift_subgoal_rr_aux5_1:
      "bins = BPF_ALU64 BPF_LSH dst (SOReg src) \<Longrightarrow>
      xins = [Ppushl_r x64Syntax.RCX, Pmovq_rr (x64Syntax.RCX) ri,Pshlq_r rd,Ppopl x64Syntax.RCX] \<Longrightarrow>
      (BPF_OK pc rs' m' ss' is_v1 (cur_cu+1) remain_cu) = step fuel bins rs m ss is_v1 cur_cu remain_cu \<Longrightarrow>
@@ -804,6 +870,20 @@ lemma shift_subgoal_rr_aux5:
      n1  = rs dst \<Longrightarrow>
      n2  = rs src \<Longrightarrow> 
      Vlong (rs' dst) = reg' (IR (bpf_to_x64_reg dst))"
+  sorry
+
+lemma shift_subgoal_rr_aux5:
+  assumes a0:"bins = BPF_ALU64 BPF_LSH dst (SOReg src)" and
+     a1:"xins = [Ppushl_r x64Syntax.RCX, Pmovq_rr (x64Syntax.RCX) ri,Pshlq_r rd,Ppopl x64Syntax.RCX]" and
+     a2:"(BPF_OK pc rs' m' ss' is_v1 (cur_cu+1) remain_cu) = step fuel bins rs m ss is_v1 cur_cu remain_cu" and
+     a3:"Next reg' m' = interp3 xins (Next reg m)" and
+     a4:"rd = (bpf_to_x64_reg dst)" and
+     a5:"ri = (bpf_to_x64_reg src)" and
+     a6:"reg (IR rd) = Vlong n1" and
+     a7:"reg (IR ri) = Vlong n2" and
+     a8:"n1  = rs dst" and
+     a9:"n2  = rs src"
+     shows "Vlong (rs' dst) = reg' (IR (bpf_to_x64_reg dst))"
   sorry
 
 lemma shift_subgoal_rr_aux6:"
@@ -822,7 +902,7 @@ lemma test1:
   using x64_encode_decode_consistency 
   by (metis a1 a2 a3 option.sel prod.inject)
 
-value "x64_decodes 2 (Option.the(x64_encodes_suffix ([Pmovq_rr x64Syntax.RAX x64Syntax.RBX,Pnop])))"
+value "x64_decodes 0 (Option.the(x64_encodes_suffix ([Pmovq_rr x64Syntax.RAX x64Syntax.RBX,Pnop])))"
 value "x64_decodes 0 (Option.the(x64_encodes_suffix ([Pnop,Pnop])))"
 value "map snd [(1::nat,Pnop),(3::nat,Pmovq_rr x64Syntax.RAX x64Syntax.RBX)]"
 
@@ -872,394 +952,7 @@ proof -
 
 
 
- (*Vlong (rs (BPC)) = reg PC \<Longrightarrow>*)
-(*lemma ja_subgoal_aux1:
-      "bins = BPF_JA off \<Longrightarrow>
-       xins = Pjmp d \<Longrightarrow>
-       (BPF_OK pc rs' m' ss' is_v1 (cur_cu+1) remain_cu) = step fuel bins rs m ss is_v1 cur_cu remain_cu \<Longrightarrow>
-       Next reg' m' = exec_instr xins sz reg m \<Longrightarrow> 
-       d = ucast(off::i16)\<Longrightarrow>
-       pc = reg' PC"
-  apply (unfold exec_instr_def step)
-  apply simp
-  apply (unfold eval_pc_def nextinstr_def add64_def)
-  apply(simp_all)
-  apply(erule conjE)+
-  apply(cases "reg RIP", simp_all)
-  using cast_lemma4 by auto
-*)
-
-lemma ja_subgoal_aux2:"xins = Pjmp d \<Longrightarrow> Next reg' m' = exec_instr xins sz reg m \<Longrightarrow>
-       \<forall> r. reg' (IR (bpf_to_x64_reg r)) = reg (IR (bpf_to_x64_reg r))"
-  apply(unfold exec_instr_def, cases "xins", simp_all)
-  apply(unfold nextinstr_nf_def nextinstr_def add64_def) 
-  by auto
-
-lemma ja_subgoal_aux3:"bins = BPF_JA off \<Longrightarrow> (BPF_OK pc rs' m' ss' is_v1 cur_cu remain_cu) = step fuel bins rs m ss is_v1 cur_cu remain_cu \<Longrightarrow>
-       \<forall> r. rs' r = rs r"
-  by(cases "bins",simp_all)
-
-lemma ja_subgoal_generic:
-  assumes a0:"bins = BPF_JA off" and
-       a1:"per_jit_ja (ucast off) = Some bl" and
-       a2:"list_in_list bl (unat pc) l_bin" and
-       a3:"x64_decode (unat pc) l_bin = Some (length l_bin, xins)" and
-       a4:"(BPF_OK pc rs' m' ss' is_v1 (cur_cu+1) remain_cu) = step fuel bins rs m ss is_v1 cur_cu remain_cu" and
-       a5:"Next reg' m' = exec_instr xins sz reg m" and
-       a6:"(\<forall> r. Vlong (rs r) = reg (IR (bpf_to_x64_reg r)))" 
-  shows "(\<forall> r. Vlong (rs' r) = reg' (IR (bpf_to_x64_reg r)))"
-proof -
-  have b0:"xins = Pjmp (ucast off)" using x64_encode_decode_consistency per_jit_ja_def a1 a2 a3 get_relative_offset_def by fastforce
-  moreover have b2:"(\<forall> r. Vlong (rs r) = reg (IR (bpf_to_x64_reg r)))" using a6 by simp
-    have b4:"\<forall> r. reg'(IR (bpf_to_x64_reg r)) = reg (IR (bpf_to_x64_reg r))" using b0 a5 ja_subgoal_aux2 by simp
-    have b5:"\<forall> r. Vlong (rs' r) = Vlong (rs r)" using a0 a4 ja_subgoal_aux3 by simp
-    have b6:"\<forall> r. Vlong (rs r) = reg (IR (bpf_to_x64_reg r))" using a6 by blast
-    have b7:"(\<forall> r. Vlong (rs' r) = reg' (IR (bpf_to_x64_reg r)))" by(simp add:b4 b5 b6) 
-    thus ?thesis using b7 by fastforce
-  qed
-
-
-lemma load_subgoal_aux1:
-      "bins = BPF_LDX chk dst src (b_off::i16) \<Longrightarrow>
-       xins = Pmov_mr (Addrmode (Some ri) None (x_off::u32)) rd chk \<Longrightarrow>
-       rd = (bpf_to_x64_reg dst)\<Longrightarrow>
-       ri = (bpf_to_x64_reg src) \<Longrightarrow>
-       reg (IR rd) = Vlong n1 \<Longrightarrow>
-       reg (IR ri) = Vlong n2 \<Longrightarrow>
-       n1  = rs dst \<Longrightarrow>
-       n2  = rs src \<Longrightarrow>
-       (BPF_OK pc rs' mem' ss' is_v1 cur_cu remain_cu) = step fuel bins rs mem ss is_v1 cur_cu remain_cu \<Longrightarrow>
-       Next reg' m'  = exec_instr xins sz reg m \<Longrightarrow> 
-       m = mem \<Longrightarrow>
-       m' = mem'"
-  apply (unfold exec_instr_def step)
-  apply(cases xins)
-  apply simp_all
-  apply (unfold eval_load_def Let_def cast_lemma6, simp_all)
-  apply (simp add: exec_load_def eval_addrmode64_def add64_def nextinstr_nf_def nextinstr_def)
-  by (metis (mono_tags, lifting) bpf_state.distinct(1) bpf_state.inject option.case_eq_if outcome.distinct(1) outcome.inject)
-
-lemma load_subgoal_aux2_1:
-  assumes a0:"bins = BPF_LDX chk dst src b_off" and 
-          a1:"step fuel bins rs mem ss is_v1 cur_cu remain_cu = result"
-        shows "result = (BPF_OK pc rs' mem' ss' is_v1 (cur_cu+1) remain_cu) \<longrightarrow> Mem.loadv chk mem (Vlong (eval_snd_op_u64 (SOReg src) rs + scast b_off)) \<noteq> Some Vundef"
-proof (rule ccontr)
-  assume a2:"\<not> (result = (BPF_OK pc rs' mem' ss' is_v1 (cur_cu+1) remain_cu) \<longrightarrow> (Mem.loadv chk mem (Vlong (eval_snd_op_u64 (SOReg src) rs + scast b_off)) \<noteq> Some Vundef))"
-  let ?x = "eval_snd_op_u64 (SOReg src) rs + scast b_off"
-  let ?tmp = "Mem.loadv chk mem (Vlong ?x)"
-  let ?res_ok = "(BPF_OK pc rs' mem' ss' is_v1 (cur_cu+1) remain_cu)"
-  have a3:"\<not> (\<not> result = ?res_ok \<or> (?tmp \<noteq> Some Vundef))" using imp_conv_disj a2 by blast
-  have a4:"result = ?res_ok \<and> ?tmp = Some Vundef" using a3 by simp
-   then show "False"
-   proof
-     have b0:"?tmp = Some Vundef" using a4 conjE by simp
-     have b1:"eval_load chk dst src b_off rs mem = None"  using eval_load_def b0 by simp
-     have b2: "step fuel bins rs mem ss is_v1 cur_cu remain_cu = BPF_EFlag"using a0 b1 eval_load_def by simp
-     thus "False" using b2 
-       by (metis a1 a4 bpf_state.distinct(3))
-   qed
- qed
-
-lemma load_subgoal_aux2_2:
-  assumes a0:"bins = BPF_LDX chk dst src b_off" and 
-          a1:"step fuel bins rs mem ss is_v1 cur_cu remain_cu = result"
-        shows "result = (BPF_OK pc rs' mem' ss' is_v1 (cur_cu+1) remain_cu) \<longrightarrow> Mem.loadv chk mem (Vlong (eval_snd_op_u64 (SOReg src) rs + scast b_off)) \<noteq> None"
-proof (rule ccontr)
-  assume a2:"\<not> (result = (BPF_OK pc rs' mem' ss' is_v1 (cur_cu+1) remain_cu) \<longrightarrow> (Mem.loadv chk mem (Vlong (eval_snd_op_u64 (SOReg src) rs + scast b_off)) \<noteq> None))"
-  let ?x = "eval_snd_op_u64 (SOReg src) rs + scast b_off"
-  let ?tmp = "Mem.loadv chk mem (Vlong ?x)"
-  let ?res_ok = "(BPF_OK pc rs' mem' ss' is_v1 (cur_cu+1) remain_cu)"
-  have a3:"\<not> (\<not> result = ?res_ok \<or> (?tmp \<noteq> None))" using imp_conv_disj a2 by blast
-  have a4:"result = ?res_ok \<and> ?tmp = None" using a3 by simp
-   then show "False"
-   proof
-     have b0:"?tmp = None" using a4 conjE by simp
-     have b1:"eval_load chk dst src b_off rs mem = None"  using eval_load_def b0 by simp
-     have b2: "step fuel bins rs mem ss is_v1 cur_cu remain_cu = BPF_EFlag"using a0 b1 eval_load_def by simp
-     thus "False" using b2 
-       using a1 a4 by auto
-   qed
- qed
-
-lemma load_subgoal_aux2_3:
-  assumes a0:"bins = BPF_LDX chk dst src b_off" and 
-          a1:"step fuel bins rs mem ss is_v1 cur_cu remain_cu = result"
-        shows "result = (BPF_OK pc rs' mem' ss' is_v1 (cur_cu+1) remain_cu) \<longrightarrow> Mem.loadv chk mem (Vlong (eval_snd_op_u64 (SOReg src) rs + scast b_off)) \<notin> {None, Some Vundef} "
-  using load_subgoal_aux2_1 load_subgoal_aux2_2 a0 a1 by auto
-
-lemma load_subgoal_aux2_4:
-  assumes a0:"bins = BPF_LDX chk dst src b_off" and 
-          a1:"step fuel bins rs mem ss is_v1 cur_cu remain_cu = result"
-        shows "result = (BPF_OK pc rs' mem' ss' is_v1 (cur_cu+1) remain_cu) \<longrightarrow> eval_load chk dst src b_off rs mem \<noteq> None"
-proof (rule ccontr)
-  assume a2:"\<not> (result = (BPF_OK pc rs' mem' ss' is_v1 (cur_cu+1) remain_cu) \<longrightarrow> eval_load chk dst src b_off rs mem \<noteq> None)"
-  let ?res_ok = "(BPF_OK pc rs' mem' ss' is_v1 (cur_cu+1) remain_cu)"
-  have a3:"\<not> (\<not> result = ?res_ok \<or> (eval_load chk dst src b_off rs mem \<noteq> None))" using imp_conv_disj a2 by blast
-  have a4:"result = ?res_ok \<and> (eval_load chk dst src b_off rs mem = None)" using a3 by simp
-   then show "False"
-   proof
-     have b1:"eval_load chk dst src b_off rs mem = None" using a4 conjE by simp
-     have b2: "step fuel bins rs mem ss is_v1 cur_cu remain_cu = BPF_EFlag"using a0 b1 eval_load_def by simp
-     thus "False" using b2 a1 a0 a2 by auto
-   qed
- qed
-
-(*lemma load_subgoal_aux2:
-      "bins = BPF_LDX chk dst src (b_off::i16) \<Longrightarrow>
-       xins = Pmov_mr (Addrmode (Some ri) None (x_off::u32)) rd chk \<Longrightarrow>
-       rd = (bpf_to_x64_reg dst)\<Longrightarrow>
-       ri = (bpf_to_x64_reg src) \<Longrightarrow>
-       reg (IR rd) = Vlong n1 \<Longrightarrow>
-       reg (IR ri) = Vlong n2 \<Longrightarrow>
-       n1  = rs dst \<Longrightarrow>
-       n2  = rs src \<Longrightarrow>
-       b_off = scast x_off \<Longrightarrow>
-       (BPF_OK pc rs' mem' ss' is_v1 cur_cu remain_cu) = step fuel bins rs mem ss is_v1 cur_cu remain_cu \<Longrightarrow>
-       Next reg' m'  = exec_instr xins sz reg m \<Longrightarrow> 
-       m = mem \<Longrightarrow>
-       Mem.loadv chk mem (Vlong (eval_snd_op_u64 (SOReg src) rs + scast (scast b_off)))\<noteq> None \<Longrightarrow>
-       scast x_off = scast (scast x_off) \<Longrightarrow>
-       Vlong (rs' dst) = reg' (IR (bpf_to_x64_reg dst))"
-  apply (unfold exec_instr_def step)
-  apply(cases xins)
-  apply simp_all
-  apply (simp add: exec_load_def eval_addrmode64_def add64_def nextinstr_nf_def nextinstr_def)
-  apply (cases "loadv chk mem (Vlong (rs src + scast x_off))")
-   apply simp
-  apply (cases "loadv chk mem (Vlong (rs src + scast (scast x_off)))")
-  apply simp_all
-  using  load_subgoal_aux2_1
-*)
-
-
-lemma load_subgoal_rr_aux2:
-  assumes a0:"bins = BPF_LDX chk dst src b_off" and
-       a1:"xins = Pmov_mr (Addrmode (Some ri) None x_off) rd chk" and
-       a2:"rd = (bpf_to_x64_reg dst)" and
-       a3:"ri = (bpf_to_x64_reg src)" and
-       a4:"reg (IR rd) = Vlong n1" and
-       a5:"reg (IR ri) = Vlong n2" and
-       a6:"n1 = rs dst" and
-       a7:"n2 = rs dst" and
-       a8:"x_off = ucast b_off " and
-       a9:"(BPF_OK pc rs' mem' ss' is_v1 (cur_cu+1) remain_cu) = step fuel bins rs mem ss is_v1 cur_cu remain_cu" and
-       a10:"Next reg' m' = exec_instr xins sz reg m" and
-       a11:"m = mem" 
-       shows "Vlong (rs' dst) = reg' (IR (bpf_to_x64_reg dst))"
-proof-
-  let ?t = "Addrmode (Some (bpf_to_x64_reg src)) None x_off"
-  have "xins = Pmov_mr ?t rd chk" using Orderings.ord.ord_less_eq_trans Extraction.exE_realizer a0 apply simp
-    using a1 a3 by fastforce
-  let ?x = "eval_snd_op_u64 (SOReg src) rs + scast b_off"
-  let ?tmp = "Mem.loadv chk mem (Vlong ?x)"
-  have b0:"step fuel bins rs mem ss is_v1 cur_cu remain_cu = (BPF_OK pc rs' mem' ss' is_v1 (cur_cu+1) remain_cu) \<longrightarrow> ?tmp \<noteq> None" 
-    using load_subgoal_aux2_2 using a0 a11 by blast
-  have b1:"?tmp \<noteq> None" using b0 a9 by simp
-  have b2:"Next reg' m' = exec_load sz chk m ?t reg (IR (bpf_to_x64_reg dst))" using exec_instr_def a1 apply (cases "xins") 
-                        apply blast apply simp_all by (simp add: a10 a2 a3)
-  have b3:"Next reg' m' = (case loadv chk m (eval_addrmode64 (?t) reg) 
-           of None \<Rightarrow> Stuck | Some (v::val) \<Rightarrow> Next (nextinstr_nf sz (reg(IR (bpf_to_x64_reg dst) := v))) m) "
-    using exec_load_def by (simp add: b2)
-  (*have b4:"Next reg' m' = (case loadv chk m (Vlong (rs src + scast x_off)) of None \<Rightarrow> Stuck
-        | Some (v::val) \<Rightarrow> Next (nextinstr_nf sz (reg(IR (bpf_to_x64_reg dst) := v))) m)"
-    using eval_addrmode64_def b3 add64_def nextinstr_nf_def using a3 a5 a7 sorry*)
-  have b4:"Next reg' m' = (case loadv chk m (Vlong (rs src + scast x_off)) of None \<Rightarrow> Stuck | 
-    Some (v::val) \<Rightarrow> Next (nextinstr_nf sz (reg(IR (bpf_to_x64_reg dst) := v))) m)" 
-    using exec_load_def eval_addrmode64_def b3 add64_def nextinstr_nf_def nextinstr_def a3 a5 a7 a11 sorry
-  have b5:"Next reg' m' = Next (nextinstr_nf sz (reg(IR (bpf_to_x64_reg dst) := Option.the(?tmp)))) m" using b4 b1 apply (cases "bins")
-    apply simp_all using a0  apply simp_all using a8 option.sel sorry
-  have b6:" reg'(IR (bpf_to_x64_reg dst)) = Option.the(?tmp)" using nextinstr_nf_def nextinstr_def b5 by simp
-  have c0:"eval_load chk dst src b_off rs mem \<noteq> None" using eval_load_def a0 load_subgoal_aux2_4 a9 by metis
-  let ?rss' = "eval_load chk dst src b_off rs mem"
- (*have c1_1:"?tmp  \<noteq> None \<or> ?tmp \<noteq> Some Vundef" using a9 load_subgoal_aux2_3 by blast
-  let "?tmpd" = "Option.the ?tmp"
-  have " \<exists> x y. eval_load chk dst src b_off rs mem \<noteq> None \<longrightarrow> ?tmp = Some (Vlong x) \<or> ?tmp = Some (Vint y) " using c1_1 eval_load_def impI *)
-(*
-  fix v1 assume "?tmp = Some(Vlong v1)" 
-  have c1_1:"(Option.the(?rss') dst) = v1" using a0 a9 the_def eval_load_def Let_def 
-    using loadv (chk) (mem) (Vlong (eval_snd_op_u64 (SOReg (src)) (rs) + scast (b_off))) = Some (Vlong (v1)) by force
-  fix v2 assume "?tmp = Some(Vint v2)" 
-  have c1_2:"(Option.the(?rss') dst) = ucast v2" using a0 a9 the_def eval_load_def Let_def 
-    using loadv (chk) (mem) (Vlong (eval_snd_op_u64 (SOReg (src)) (rs) + scast (b_off))) = Some (Vint (v2)) by force
-  fix v3 assume "?tmp = None" 
- *)
-  have c1:"Vlong ((Option.the(?rss') dst)) = Option.the(?tmp)" (*using a0 a9 the_def eval_load_def Let_def c0 cast_lemma6*)
-  proof (cases ?tmp)
-    case None
-    have d1:"eval_load chk dst src b_off rs mem = None" using eval_load_def 
-      using None b1 by blast
-    then show ?thesis using c0 d1 by simp
-  next
-    case (Some a)
-      then show ?thesis 
-    proof(cases a)
-      case Vundef
-        have d1:"eval_load chk dst src b_off rs mem = None" using eval_load_def 
-          using Some Vundef by auto
-          then show ?thesis using c0 d1 by simp
-       next
-         case (Vlong b)
-         then show ?thesis using eval_load_def
-           using Some by auto
-       next
-         case (Vint c)
-         then show ?thesis using eval_load_def Let_def c0 sorry
-           by simp
-       next
-         case (Vbyte c)
-         have d1:"eval_load chk dst src b_off rs mem = None" using eval_load_def 
-          using Some Vbyte by auto
-          then show ?thesis using c0 d1 by simp
-       next
-         case (Vshort c)
-         have d1:"eval_load chk dst src b_off rs mem = None" using eval_load_def 
-           using Some Vshort by auto
-           then show ?thesis using c0 d1 by simp
-       qed
-     qed
-  have c3:"Option.the(?rss')dst = rs' dst" using the_def sorry
-  have c4:"Vlong (rs' dst) = Option.the(?tmp)" using c3 c1 by simp
-  thus ?thesis using c4 b6 by simp
-qed
-
-
-lemma load_subgoal_rr_aux3_1:"xins = Pmov_mr (Addrmode (Some src) None (b_off)) dst chk \<Longrightarrow> 
-  Next reg' m' = exec_instr xins sz reg m \<Longrightarrow> \<forall> r \<noteq> dst. reg' (IR r) = reg (IR r)"
-  apply(unfold exec_instr_def, cases "xins", simp_all)
-  apply(unfold exec_load_def eval_addrmode64_def nextinstr_nf_def nextinstr_def add64_def) 
-  apply(cases "Addrmode (Some src) None b_off")
-  subgoal for x1 x2 x3 apply(simp_all) apply(cases x1,simp_all)
-    apply (cases "reg (IR src)",simp_all) 
-        apply(cases "loadv chk m Vundef",simp_all)
-    subgoal for a apply(cases "loadv chk m Vundef",simp_all)
-      done
-    subgoal for b apply(cases "loadv chk m Vundef",simp_all)
-      done
-    subgoal for c apply(cases "loadv chk m Vundef",simp_all)
-      done
-    subgoal for x4 apply(cases "loadv chk m (Vlong (x4 + scast x3))",simp_all)
-      done
-    done
-  done
-
-lemma loadq_subgoal_rr_aux3: 
-  assumes a0:"xins = Pmov_mr (Addrmode (Some (bpf_to_x64_reg src)) None (ucast (b_off))) (bpf_to_x64_reg dst) chk" and
-          a1:"Next reg' m' = exec_instr xins sz reg m" 
-        shows " \<forall> r \<noteq> dst. reg' (IR (bpf_to_x64_reg r)) = reg (IR (bpf_to_x64_reg r))"
- using cast_lemma6 a0 by (metis a1 bpf_to_x64_reg_corr load_subgoal_rr_aux3_1)
-
-lemma loadq_subgoal_rr_aux4:"bins = BPF_LDX chk dst src b_off \<Longrightarrow> (BPF_OK pc rs' m' ss' is_v1 (cur_cu+1) remain_cu) = step fuel bins rs m ss is_v1 cur_cu remain_cu \<Longrightarrow>
-       \<forall> r \<noteq> dst. rs' r = rs r"
-  apply(cases "bins",simp_all)
-  apply(unfold eval_load_def,simp)
-  apply(cases "loadv chk m (Vlong (rs src + scast b_off))" ,simp_all)
-  subgoal for a apply(cases a)
-  by simp_all
-  done
-
-lemma loadq_subgoal_rr_generic:
-  assumes a0:"bins = BPF_LDX chk dst src b_off" and
-       a1:"per_jit_load_reg64 dst src chk b_off = Some bl" and
-       a2:"list_in_list bl (unat pc) l_bin" and
-       a3:"x64_decode (unat pc) l_bin = Some (length l_bin, xins)" and
-       a4:"(BPF_OK pc rs' mem' ss' is_v1 (cur_cu+1) remain_cu) = step fuel bins rs mem ss is_v1 cur_cu remain_cu" and
-       a5:"Next reg' m' = exec_instr xins sz reg m" and
-       a6:"(\<forall> r. Vlong (rs r) = reg (IR (bpf_to_x64_reg r)))" and
-       a7:"m = mem"
-  shows "(\<forall> r. Vlong (rs' r) = reg' (IR (bpf_to_x64_reg r)))"
-proof -
-  have b0:"xins = Pmov_mr (Addrmode (Some (bpf_to_x64_reg src)) None (ucast (b_off))) (bpf_to_x64_reg dst) chk" using x64_encode_decode_consistency per_jit_load_reg64_def a1 a2 a3 by fastforce
-    moreover have b1:"Vlong (rs dst) = reg (IR (bpf_to_x64_reg dst))" using a6 spec by simp
-    moreover have b2:"Vlong (rs src) = reg (IR (bpf_to_x64_reg src))" using a6 spec by simp
-    hence b3:"Vlong (rs' dst) = reg' (IR (bpf_to_x64_reg dst))" using load_subgoal_rr_aux2 b0 b1 b2 a0 a1 a2 a3 a4 a5 a6 a7 sorry
-    have b4:"\<forall> r \<noteq> dst. reg'(IR (bpf_to_x64_reg r)) = reg (IR (bpf_to_x64_reg r))" using b0 a5 loadq_subgoal_rr_aux3 by blast
-    have b5:"\<forall> r \<noteq> dst. Vlong (rs' r) = Vlong (rs r)" using a0 a4 loadq_subgoal_rr_aux4 by blast
-    have b6:"\<forall> r \<noteq> dst. Vlong (rs r) = reg (IR (bpf_to_x64_reg r))" using a6 by blast
-    have b7:"(\<forall> r \<noteq> dst. Vlong (rs' r) = reg' (IR (bpf_to_x64_reg r)))" by(simp add:b4 b5 b6) 
-    thus ?thesis using b3 by fastforce
-  qed
-
-lemma addl_subgoal_rr:
-      "bins = BPF_ALU BPF_ADD dst (SOReg src) \<Longrightarrow>
-       xins = Paddl_rr rd ri \<Longrightarrow>
-       (BPF_OK pc rs' m' ss' is_v1 (cur_cu+1) remain_cu) = step fuel bins rs m ss is_v1 cur_cu remain_cu \<Longrightarrow>
-       Next reg' m'  = exec_instr xins sz reg m \<Longrightarrow> 
-       rd = bpf_to_x64_reg dst \<Longrightarrow>
-       ri = bpf_to_x64_reg src \<Longrightarrow>
-       reg (IR rd) = Vint n1 \<Longrightarrow>
-       reg (IR ri) = Vint n2 \<Longrightarrow>
-       ucast n1 = rs dst \<Longrightarrow>
-       ucast n2  = rs src \<Longrightarrow>
-       reg' (IR rd) = Vint n3 \<Longrightarrow>
-       ucast n3 = rs'dst"
-  apply (unfold exec_instr_def step)
-  apply simp
-  apply (unfold eval_alu32_def)
-  apply (unfold eval_alu32_aux1_def)
-  apply (unfold Let_def)
-  apply (unfold add64_def add32_def)
-  apply (unfold nextinstr_nf_def nextinstr_def eval_reg_def)
-  apply simp
-  apply (unfold add64_def)
-  apply (erule conjE)
-  using cast_lemma2
+ 
   
-
-
-
-lemma addl_subgoal_ri:
-      "bins = BPF_ALU BPF_ADD dst (SOImm src) \<Longrightarrow>
-       xins = Paddl_ri rd imm \<Longrightarrow>
-       (BPF_OK pc rs' m' ss' is_v1 (cur_cu+1) remain_cu) = step fuel bins rs m ss is_v1 cur_cu remain_cu \<Longrightarrow>
-       Next reg' m' = exec_instr xins sz reg m \<Longrightarrow> 
-       rd = bpf_to_x64_reg dst \<Longrightarrow>
-       imm = ucast (src) \<Longrightarrow>
-       reg (IR rd) = Vint n1 \<Longrightarrow>
-       ucast n1  = rs dst \<Longrightarrow>
-       reg' (IR rd) = Vint n3 \<Longrightarrow>
-       ucast n3 = rs'dst"
-  apply (unfold exec_instr_def step)
-  apply simp
-  apply (unfold eval_alu32_def)
-  apply (cases BPF_ADD, simp_all)
-  apply (unfold eval_alu32_aux1_def)
-  apply (unfold Let_def)
-  apply (cases BPF_ADD, simp_all)
-  apply (unfold add64_def add32_def)
-  apply (unfold nextinstr_nf_def nextinstr_def eval_reg_def)
-  apply simp
-  apply (unfold add64_def)
-  apply (erule conjE)
-  using cast_lemma2 
-  by metis
-
-
-lemma subl_subgoal_ri:
-      "bins = BPF_ALU BPF_SUB dst (SOImm src) \<Longrightarrow>
-       xins = Psubl_ri rd imm \<Longrightarrow>
-       (BPF_OK pc rs' m' ss' is_v1 (cur_cu+1) remain_cu) = step fuel bins rs m ss is_v1 cur_cu remain_cu \<Longrightarrow>
-       Next reg' m'  = exec_instr xins sz reg m \<Longrightarrow> 
-       rd = bpf_to_x64_reg dst \<Longrightarrow>
-       imm = ucast (src) \<Longrightarrow>
-       reg (IR rd) = Vint n1 \<Longrightarrow>
-       ucast n1  = rs dst \<Longrightarrow>
-       reg' (IR rd) = Vint n3 \<Longrightarrow>
-       ucast n3 = rs'dst"
-  apply (unfold exec_instr_def step)
-  apply simp
-  apply (unfold eval_alu32_def)
-  apply (cases BPF_SUB, simp_all)
-  apply (unfold eval_alu32_aux1_def)
-  apply (unfold Let_def)
-  apply (cases BPF_SUB, simp_all)
-  apply (unfold sub32_def )
-  apply (unfold nextinstr_nf_def nextinstr_def eval_reg_def)
-  apply simp
-  apply (unfold add64_def)
-  apply (erule conjE)
-  apply (cases "is_v1", simp_all)
-  apply (cases "is_v1", simp_all)
-  using cast_lemma2 
-  sorry
 
 end
