theory/bpfConsistencyAux2.thy
@@ -1,0 +1,613 @@
+theory bpfConsistencyAux2
+  imports Main Interpreter x64Semantics 
+  x64Assembler x64DecodeProof Mem JITCommType
+
+begin
+(*Vlong (rs (BPC)) = reg PC \<Longrightarrow>*)
+(*lemma ja_subgoal_aux1:
+      "bins = BPF_JA off \<Longrightarrow>
+       xins = Pjmp d \<Longrightarrow>
+       (BPF_OK pc rs' m' ss' is_v1 (cur_cu+1) remain_cu) = step fuel bins rs m ss is_v1 cur_cu remain_cu \<Longrightarrow>
+       Next reg' m' = exec_instr xins sz reg m \<Longrightarrow> 
+       d = ucast(off::i16)\<Longrightarrow>
+       pc = reg' PC"
+  apply (unfold exec_instr_def step)
+  apply simp
+  apply (unfold eval_pc_def nextinstr_def add64_def)
+  apply(simp_all)
+  apply(erule conjE)+
+  apply(cases "reg RIP", simp_all)
+  using cast_lemma4 by auto
+*)
+
+lemma ja_subgoal_aux2:"xins = Pjmp d \<Longrightarrow> Next reg' m' = exec_instr xins sz reg m \<Longrightarrow>
+       \<forall> r. reg' (IR (bpf_to_x64_reg r)) = reg (IR (bpf_to_x64_reg r))"
+  apply(unfold exec_instr_def, cases "xins", simp_all)
+  apply(unfold nextinstr_nf_def nextinstr_def add64_def) 
+  by auto
+
+lemma ja_subgoal_aux3:"bins = BPF_JA off \<Longrightarrow> (BPF_OK pc rs' m' ss' is_v1 cur_cu remain_cu) = step fuel bins rs m ss is_v1 cur_cu remain_cu \<Longrightarrow>
+       \<forall> r. rs' r = rs r"
+  by(cases "bins",simp_all)
+
+lemma ja_subgoal_generic:
+  assumes a0:"bins = BPF_JA off" and
+       a1:"per_jit_ja (ucast off) = Some bl" and
+       a2:"list_in_list bl (unat pc) l_bin" and
+       a3:"x64_decode (unat pc) l_bin = Some (length l_bin, xins)" and
+       a4:"(BPF_OK pc rs' m' ss' is_v1 (cur_cu+1) remain_cu) = step fuel bins rs m ss is_v1 cur_cu remain_cu" and
+       a5:"Next reg' m' = exec_instr xins sz reg m" and
+       a6:"(\<forall> r. Vlong (rs r) = reg (IR (bpf_to_x64_reg r)))" 
+  shows "(\<forall> r. Vlong (rs' r) = reg' (IR (bpf_to_x64_reg r)))"
+proof -
+  have b0:"xins = Pjmp (ucast off)" using x64_encode_decode_consistency per_jit_ja_def a1 a2 a3 get_relative_offset_def by fastforce
+  moreover have b2:"(\<forall> r. Vlong (rs r) = reg (IR (bpf_to_x64_reg r)))" using a6 by simp
+    have b4:"\<forall> r. reg'(IR (bpf_to_x64_reg r)) = reg (IR (bpf_to_x64_reg r))" using b0 a5 ja_subgoal_aux2 by simp
+    have b5:"\<forall> r. Vlong (rs' r) = Vlong (rs r)" using a0 a4 ja_subgoal_aux3 by simp
+    have b6:"\<forall> r. Vlong (rs r) = reg (IR (bpf_to_x64_reg r))" using a6 by blast
+    have b7:"(\<forall> r. Vlong (rs' r) = reg' (IR (bpf_to_x64_reg r)))" by(simp add:b4 b5 b6) 
+    thus ?thesis using b7 by fastforce
+  qed
+
+
+lemma load_subgoal_aux1:
+      "bins = BPF_LDX chk dst src (b_off::i16) \<Longrightarrow>
+       xins = Pmov_mr (Addrmode (Some ri) None (x_off::u32)) rd chk \<Longrightarrow>
+       rd = (bpf_to_x64_reg dst)\<Longrightarrow>
+       ri = (bpf_to_x64_reg src) \<Longrightarrow>
+       reg (IR rd) = Vlong n1 \<Longrightarrow>
+       reg (IR ri) = Vlong n2 \<Longrightarrow>
+       n1  = rs dst \<Longrightarrow>
+       n2  = rs src \<Longrightarrow>
+       (BPF_OK pc rs' mem' ss' is_v1 cur_cu remain_cu) = step fuel bins rs mem ss is_v1 cur_cu remain_cu \<Longrightarrow>
+       Next reg' m'  = exec_instr xins sz reg m \<Longrightarrow> 
+       m = mem \<Longrightarrow>
+       m' = mem'"
+  apply (unfold exec_instr_def step)
+  apply(cases xins)
+  apply simp_all
+  apply (unfold eval_load_def Let_def cast_lemma6, simp_all)
+  apply (simp add: exec_load_def eval_addrmode64_def add64_def nextinstr_nf_def nextinstr_def)
+  by (metis (mono_tags, lifting) bpf_state.distinct(1) bpf_state.inject option.case_eq_if outcome.distinct(1) outcome.inject)
+
+lemma load_subgoal_aux2_1:
+  assumes a0:"bins = BPF_LDX chk dst src b_off" and 
+          a1:"step fuel bins rs mem ss is_v1 cur_cu remain_cu = result"
+        shows "result = (BPF_OK pc rs' mem' ss' is_v1 (cur_cu+1) remain_cu) \<longrightarrow> Mem.loadv chk mem (Vlong (eval_snd_op_u64 (SOReg src) rs + scast b_off)) \<noteq> Some Vundef"
+proof (rule ccontr)
+  assume a2:"\<not> (result = (BPF_OK pc rs' mem' ss' is_v1 (cur_cu+1) remain_cu) \<longrightarrow> (Mem.loadv chk mem (Vlong (eval_snd_op_u64 (SOReg src) rs + scast b_off)) \<noteq> Some Vundef))"
+  let ?x = "eval_snd_op_u64 (SOReg src) rs + scast b_off"
+  let ?tmp = "Mem.loadv chk mem (Vlong ?x)"
+  let ?res_ok = "(BPF_OK pc rs' mem' ss' is_v1 (cur_cu+1) remain_cu)"
+  have a3:"\<not> (\<not> result = ?res_ok \<or> (?tmp \<noteq> Some Vundef))" using imp_conv_disj a2 by blast
+  have a4:"result = ?res_ok \<and> ?tmp = Some Vundef" using a3 by simp
+   then show "False"
+   proof
+     have b0:"?tmp = Some Vundef" using a4 conjE by simp
+     have b1:"eval_load chk dst src b_off rs mem = None"  using eval_load_def b0 by simp
+     have b2: "step fuel bins rs mem ss is_v1 cur_cu remain_cu = BPF_EFlag"using a0 b1 eval_load_def by simp
+     thus "False" using b2 
+       by (metis a1 a4 bpf_state.distinct(3))
+   qed
+ qed
+
+lemma load_subgoal_aux2_2:
+  assumes a0:"bins = BPF_LDX chk dst src b_off" and 
+          a1:"step fuel bins rs mem ss is_v1 cur_cu remain_cu = result"
+        shows "result = (BPF_OK pc rs' mem' ss' is_v1 (cur_cu+1) remain_cu) \<longrightarrow> Mem.loadv chk mem (Vlong (eval_snd_op_u64 (SOReg src) rs + scast b_off)) \<noteq> None"
+proof (rule ccontr)
+  assume a2:"\<not> (result = (BPF_OK pc rs' mem' ss' is_v1 (cur_cu+1) remain_cu) \<longrightarrow> (Mem.loadv chk mem (Vlong (eval_snd_op_u64 (SOReg src) rs + scast b_off)) \<noteq> None))"
+  let ?x = "eval_snd_op_u64 (SOReg src) rs + scast b_off"
+  let ?tmp = "Mem.loadv chk mem (Vlong ?x)"
+  let ?res_ok = "(BPF_OK pc rs' mem' ss' is_v1 (cur_cu+1) remain_cu)"
+  have a3:"\<not> (\<not> result = ?res_ok \<or> (?tmp \<noteq> None))" using imp_conv_disj a2 by blast
+  have a4:"result = ?res_ok \<and> ?tmp = None" using a3 by simp
+   then show "False"
+   proof
+     have b0:"?tmp = None" using a4 conjE by simp
+     have b1:"eval_load chk dst src b_off rs mem = None"  using eval_load_def b0 by simp
+     have b2: "step fuel bins rs mem ss is_v1 cur_cu remain_cu = BPF_EFlag"using a0 b1 eval_load_def by simp
+     thus "False" using b2 
+       using a1 a4 by auto
+   qed
+ qed
+
+lemma load_subgoal_aux2_3:
+  assumes a0:"bins = BPF_LDX chk dst src b_off" and 
+          a1:"step fuel bins rs mem ss is_v1 cur_cu remain_cu = result"
+        shows "result = (BPF_OK pc rs' mem' ss' is_v1 (cur_cu+1) remain_cu) \<longrightarrow> Mem.loadv chk mem (Vlong (eval_snd_op_u64 (SOReg src) rs + scast b_off)) \<notin> {None, Some Vundef} "
+  using load_subgoal_aux2_1 load_subgoal_aux2_2 a0 a1 by auto
+
+lemma load_subgoal_aux2_4:
+  assumes a0:"bins = BPF_LDX chk dst src b_off" and 
+          a1:"step fuel bins rs mem ss is_v1 cur_cu remain_cu = result"
+        shows "result = (BPF_OK pc rs' mem' ss' is_v1 (cur_cu+1) remain_cu) \<longrightarrow> eval_load chk dst src b_off rs mem \<noteq> None"
+proof (rule ccontr)
+  assume a2:"\<not> (result = (BPF_OK pc rs' mem' ss' is_v1 (cur_cu+1) remain_cu) \<longrightarrow> eval_load chk dst src b_off rs mem \<noteq> None)"
+  let ?res_ok = "(BPF_OK pc rs' mem' ss' is_v1 (cur_cu+1) remain_cu)"
+  have a3:"\<not> (\<not> result = ?res_ok \<or> (eval_load chk dst src b_off rs mem \<noteq> None))" using imp_conv_disj a2 by blast
+  have a4:"result = ?res_ok \<and> (eval_load chk dst src b_off rs mem = None)" using a3 by simp
+   then show "False"
+   proof
+     have b1:"eval_load chk dst src b_off rs mem = None" using a4 conjE by simp
+     have b2: "step fuel bins rs mem ss is_v1 cur_cu remain_cu = BPF_EFlag"using a0 b1 eval_load_def by simp
+     thus "False" using b2 a1 a0 a2 by auto
+   qed
+ qed
+
+(*lemma load_subgoal_aux2:
+      "bins = BPF_LDX chk dst src (b_off::i16) \<Longrightarrow>
+       xins = Pmov_mr (Addrmode (Some ri) None (x_off::u32)) rd chk \<Longrightarrow>
+       rd = (bpf_to_x64_reg dst)\<Longrightarrow>
+       ri = (bpf_to_x64_reg src) \<Longrightarrow>
+       reg (IR rd) = Vlong n1 \<Longrightarrow>
+       reg (IR ri) = Vlong n2 \<Longrightarrow>
+       n1  = rs dst \<Longrightarrow>
+       n2  = rs src \<Longrightarrow>
+       b_off = scast x_off \<Longrightarrow>
+       (BPF_OK pc rs' mem' ss' is_v1 cur_cu remain_cu) = step fuel bins rs mem ss is_v1 cur_cu remain_cu \<Longrightarrow>
+       Next reg' m'  = exec_instr xins sz reg m \<Longrightarrow> 
+       m = mem \<Longrightarrow>
+       Mem.loadv chk mem (Vlong (eval_snd_op_u64 (SOReg src) rs + scast (scast b_off)))\<noteq> None \<Longrightarrow>
+       scast x_off = scast (scast x_off) \<Longrightarrow>
+       Vlong (rs' dst) = reg' (IR (bpf_to_x64_reg dst))"
+  apply (unfold exec_instr_def step)
+  apply(cases xins)
+  apply simp_all
+  apply (simp add: exec_load_def eval_addrmode64_def add64_def nextinstr_nf_def nextinstr_def)
+  apply (cases "loadv chk mem (Vlong (rs src + scast x_off))")
+   apply simp
+  apply (cases "loadv chk mem (Vlong (rs src + scast (scast x_off)))")
+  apply simp_all
+  using  load_subgoal_aux2_1
+*)
+
+
+lemma load_subgoal_rr_aux2:
+  assumes a0:"bins = BPF_LDX chk dst src b_off" and
+       a1:"xins = Pmov_mr (Addrmode (Some ri) None x_off) rd chk" and
+       a2:"rd = (bpf_to_x64_reg dst)" and
+       a3:"ri = (bpf_to_x64_reg src)" and
+       a4:"reg (IR rd) = Vlong n1" and
+       a5:"reg (IR ri) = Vlong n2" and
+       a6:"n1 = rs dst" and
+       a7:"n2 = rs dst" and
+       a8:"x_off = ucast b_off " and
+       a9:"(BPF_OK pc rs' mem' ss' is_v1 (cur_cu+1) remain_cu) = step fuel bins rs mem ss is_v1 cur_cu remain_cu" and
+       a10:"Next reg' m' = exec_instr xins sz reg m" and
+       a11:"m = mem" 
+       shows "Vlong (rs' dst) = reg' (IR (bpf_to_x64_reg dst))"
+proof-
+  let ?t = "Addrmode (Some (bpf_to_x64_reg src)) None x_off"
+  have "xins = Pmov_mr ?t rd chk" using Orderings.ord.ord_less_eq_trans Extraction.exE_realizer a0 apply simp
+    using a1 a3 by fastforce
+  let ?x = "eval_snd_op_u64 (SOReg src) rs + scast b_off"
+  let ?tmp = "Mem.loadv chk mem (Vlong ?x)"
+  have b0:"step fuel bins rs mem ss is_v1 cur_cu remain_cu = (BPF_OK pc rs' mem' ss' is_v1 (cur_cu+1) remain_cu) \<longrightarrow> ?tmp \<noteq> None" 
+    using load_subgoal_aux2_2 using a0 a11 by blast
+  have b1:"?tmp \<noteq> None" using b0 a9 by simp
+  have b2:"Next reg' m' = exec_load sz chk m ?t reg (IR (bpf_to_x64_reg dst))" using exec_instr_def a1 apply (cases "xins") 
+                        apply blast apply simp_all by (simp add: a10 a2 a3)
+  have b3:"Next reg' m' = (case loadv chk m (eval_addrmode64 (?t) reg) 
+           of None \<Rightarrow> Stuck | Some (v::val) \<Rightarrow> Next (nextinstr_nf sz (reg(IR (bpf_to_x64_reg dst) := v))) m) "
+    using exec_load_def by (simp add: b2)
+  (*have b4:"Next reg' m' = (case loadv chk m (Vlong (rs src + scast x_off)) of None \<Rightarrow> Stuck
+        | Some (v::val) \<Rightarrow> Next (nextinstr_nf sz (reg(IR (bpf_to_x64_reg dst) := v))) m)"
+    using eval_addrmode64_def b3 add64_def nextinstr_nf_def using a3 a5 a7 sorry*)
+  have b4:"Next reg' m' = (case loadv chk m (Vlong (rs src + scast x_off)) of None \<Rightarrow> Stuck | 
+    Some (v::val) \<Rightarrow> Next (nextinstr_nf sz (reg(IR (bpf_to_x64_reg dst) := v))) m)" 
+    using exec_load_def eval_addrmode64_def b3 add64_def nextinstr_nf_def nextinstr_def a3 a5 a7 a11 sorry
+  have b5:"Next reg' m' = Next (nextinstr_nf sz (reg(IR (bpf_to_x64_reg dst) := Option.the(?tmp)))) m" using b4 b1 apply (cases "bins")
+    apply simp_all using a0  apply simp_all using a8 option.sel sorry
+  have b6:" reg'(IR (bpf_to_x64_reg dst)) = Option.the(?tmp)" using nextinstr_nf_def nextinstr_def b5 by simp
+  have c0:"eval_load chk dst src b_off rs mem \<noteq> None" using eval_load_def a0 load_subgoal_aux2_4 a9 by metis
+  let ?rss' = "eval_load chk dst src b_off rs mem"
+ (*have c1_1:"?tmp  \<noteq> None \<or> ?tmp \<noteq> Some Vundef" using a9 load_subgoal_aux2_3 by blast
+  let "?tmpd" = "Option.the ?tmp"
+  have " \<exists> x y. eval_load chk dst src b_off rs mem \<noteq> None \<longrightarrow> ?tmp = Some (Vlong x) \<or> ?tmp = Some (Vint y) " using c1_1 eval_load_def impI *)
+(*
+  fix v1 assume "?tmp = Some(Vlong v1)" 
+  have c1_1:"(Option.the(?rss') dst) = v1" using a0 a9 the_def eval_load_def Let_def 
+    using loadv (chk) (mem) (Vlong (eval_snd_op_u64 (SOReg (src)) (rs) + scast (b_off))) = Some (Vlong (v1)) by force
+  fix v2 assume "?tmp = Some(Vint v2)" 
+  have c1_2:"(Option.the(?rss') dst) = ucast v2" using a0 a9 the_def eval_load_def Let_def 
+    using loadv (chk) (mem) (Vlong (eval_snd_op_u64 (SOReg (src)) (rs) + scast (b_off))) = Some (Vint (v2)) by force
+  fix v3 assume "?tmp = None" 
+ *)
+  have c1:"Vlong ((Option.the(?rss') dst)) = Option.the(?tmp)" (*using a0 a9 the_def eval_load_def Let_def c0 cast_lemma6*)
+  proof (cases ?tmp)
+    case None
+    have d1:"eval_load chk dst src b_off rs mem = None" using eval_load_def 
+      using None b1 by blast
+    then show ?thesis using c0 d1 by simp
+  next
+    case (Some a)
+      then show ?thesis 
+    proof(cases a)
+      case Vundef
+        have d1:"eval_load chk dst src b_off rs mem = None" using eval_load_def 
+          using Some Vundef by auto
+          then show ?thesis using c0 d1 by simp
+       next
+         case (Vlong b)
+         then show ?thesis using eval_load_def
+           using Some by auto
+       next
+         case (Vint c)
+         then show ?thesis using eval_load_def Let_def c0 sorry
+           by simp
+       next
+         case (Vbyte c)
+         have d1:"eval_load chk dst src b_off rs mem = None" using eval_load_def 
+          using Some Vbyte by auto
+          then show ?thesis using c0 d1 by simp
+       next
+         case (Vshort c)
+         have d1:"eval_load chk dst src b_off rs mem = None" using eval_load_def 
+           using Some Vshort by auto
+           then show ?thesis using c0 d1 by simp
+       qed
+     qed
+  have c3:"Option.the(?rss')dst = rs' dst" using the_def sorry
+  have c4:"Vlong (rs' dst) = Option.the(?tmp)" using c3 c1 by simp
+  thus ?thesis using c4 b6 by simp
+qed
+
+
+lemma load_subgoal_rr_aux3_1:"xins = Pmov_mr (Addrmode (Some src) None (b_off)) dst chk \<Longrightarrow> 
+  Next reg' m' = exec_instr xins sz reg m \<Longrightarrow> \<forall> r \<noteq> dst. reg' (IR r) = reg (IR r)"
+  apply(unfold exec_instr_def, cases "xins", simp_all)
+  apply(unfold exec_load_def eval_addrmode64_def nextinstr_nf_def nextinstr_def add64_def) 
+  apply(cases "Addrmode (Some src) None b_off")
+  subgoal for x1 x2 x3 apply(simp_all) apply(cases x1,simp_all)
+    apply (cases "reg (IR src)",simp_all) 
+        apply(cases "loadv chk m Vundef",simp_all)
+    subgoal for a apply(cases "loadv chk m Vundef",simp_all)
+      done
+    subgoal for b apply(cases "loadv chk m Vundef",simp_all)
+      done
+    subgoal for c apply(cases "loadv chk m Vundef",simp_all)
+      done
+    subgoal for x4 apply(cases "loadv chk m (Vlong (x4 + scast x3))",simp_all)
+      done
+    done
+  done
+
+lemma loadq_subgoal_rr_aux3: 
+  assumes a0:"xins = Pmov_mr (Addrmode (Some (bpf_to_x64_reg src)) None (ucast (b_off))) (bpf_to_x64_reg dst) chk" and
+          a1:"Next reg' m' = exec_instr xins sz reg m" 
+        shows " \<forall> r \<noteq> dst. reg' (IR (bpf_to_x64_reg r)) = reg (IR (bpf_to_x64_reg r))"
+ using cast_lemma6 a0 by (metis a1 bpf_to_x64_reg_corr load_subgoal_rr_aux3_1)
+
+lemma loadq_subgoal_rr_aux4:"bins = BPF_LDX chk dst src b_off \<Longrightarrow> (BPF_OK pc rs' m' ss' is_v1 (cur_cu+1) remain_cu) = step fuel bins rs m ss is_v1 cur_cu remain_cu \<Longrightarrow>
+       \<forall> r \<noteq> dst. rs' r = rs r"
+  apply(cases "bins",simp_all)
+  apply(unfold eval_load_def,simp)
+  apply(cases "loadv chk m (Vlong (rs src + scast b_off))" ,simp_all)
+  subgoal for a apply(cases a)
+  by simp_all
+  done
+
+lemma loadq_subgoal_rr_generic:
+  assumes a0:"bins = BPF_LDX chk dst src b_off" and
+       a1:"per_jit_load_reg64 dst src chk b_off = Some bl" and
+       a2:"list_in_list bl (unat pc) l_bin" and
+       a3:"x64_decode (unat pc) l_bin = Some (length l_bin, xins)" and
+       a4:"(BPF_OK pc rs' mem' ss' is_v1 (cur_cu+1) remain_cu) = step fuel bins rs mem ss is_v1 cur_cu remain_cu" and
+       a5:"Next reg' m' = exec_instr xins sz reg m" and
+       a6:"(\<forall> r. Vlong (rs r) = reg (IR (bpf_to_x64_reg r)))" and
+       a7:"m = mem"
+  shows "(\<forall> r. Vlong (rs' r) = reg' (IR (bpf_to_x64_reg r)))"
+proof -
+  have b0:"xins = Pmov_mr (Addrmode (Some (bpf_to_x64_reg src)) None (ucast (b_off))) (bpf_to_x64_reg dst) chk" using x64_encode_decode_consistency per_jit_load_reg64_def a1 a2 a3 by fastforce
+    moreover have b1:"Vlong (rs dst) = reg (IR (bpf_to_x64_reg dst))" using a6 spec by simp
+    moreover have b2:"Vlong (rs src) = reg (IR (bpf_to_x64_reg src))" using a6 spec by simp
+    hence b3:"Vlong (rs' dst) = reg' (IR (bpf_to_x64_reg dst))" using load_subgoal_rr_aux2 b0 b1 b2 a0 a1 a2 a3 a4 a5 a6 a7 sorry
+    have b4:"\<forall> r \<noteq> dst. reg'(IR (bpf_to_x64_reg r)) = reg (IR (bpf_to_x64_reg r))" using b0 a5 loadq_subgoal_rr_aux3 by blast
+    have b5:"\<forall> r \<noteq> dst. Vlong (rs' r) = Vlong (rs r)" using a0 a4 loadq_subgoal_rr_aux4 by blast
+    have b6:"\<forall> r \<noteq> dst. Vlong (rs r) = reg (IR (bpf_to_x64_reg r))" using a6 by blast
+    have b7:"(\<forall> r \<noteq> dst. Vlong (rs' r) = reg' (IR (bpf_to_x64_reg r)))" by(simp add:b4 b5 b6) 
+    thus ?thesis using b3 by fastforce
+  qed
+
+lemma addl_subgoal_rr:
+      "bins = BPF_ALU BPF_ADD dst (SOReg src) \<Longrightarrow>
+       xins = Paddl_rr rd ri \<Longrightarrow>
+       (BPF_OK pc rs' m' ss' is_v1 (cur_cu+1) remain_cu) = step fuel bins rs m ss is_v1 cur_cu remain_cu \<Longrightarrow>
+       Next reg' m'  = exec_instr xins sz reg m \<Longrightarrow> 
+       rd = bpf_to_x64_reg dst \<Longrightarrow>
+       ri = bpf_to_x64_reg src \<Longrightarrow>
+       reg (IR rd) = Vint n1 \<Longrightarrow>
+       reg (IR ri) = Vint n2 \<Longrightarrow>
+       ucast n1 = rs dst \<Longrightarrow>
+       ucast n2  = rs src \<Longrightarrow>
+       reg' (IR rd) = Vint n3 \<Longrightarrow>
+       ucast n3 = rs'dst"
+  apply (unfold exec_instr_def step)
+  apply simp
+  apply (unfold eval_alu32_def)
+  apply (unfold eval_alu32_aux1_def)
+  apply (unfold Let_def)
+  apply (unfold add64_def add32_def)
+  apply (unfold nextinstr_nf_def nextinstr_def eval_reg_def)
+  apply simp
+  apply (unfold add64_def)
+  apply (erule conjE)
+  using cast_lemma2
+  
+
+
+
+lemma addl_subgoal_ri:
+      "bins = BPF_ALU BPF_ADD dst (SOImm src) \<Longrightarrow>
+       xins = Paddl_ri rd imm \<Longrightarrow>
+       (BPF_OK pc rs' m' ss' is_v1 (cur_cu+1) remain_cu) = step fuel bins rs m ss is_v1 cur_cu remain_cu \<Longrightarrow>
+       Next reg' m' = exec_instr xins sz reg m \<Longrightarrow> 
+       rd = bpf_to_x64_reg dst \<Longrightarrow>
+       imm = ucast (src) \<Longrightarrow>
+       reg (IR rd) = Vint n1 \<Longrightarrow>
+       ucast n1  = rs dst \<Longrightarrow>
+       reg' (IR rd) = Vint n3 \<Longrightarrow>
+       ucast n3 = rs'dst"
+  apply (unfold exec_instr_def step)
+  apply simp
+  apply (unfold eval_alu32_def)
+  apply (cases BPF_ADD, simp_all)
+  apply (unfold eval_alu32_aux1_def)
+  apply (unfold Let_def)
+  apply (cases BPF_ADD, simp_all)
+  apply (unfold add64_def add32_def)
+  apply (unfold nextinstr_nf_def nextinstr_def eval_reg_def)
+  apply simp
+  apply (unfold add64_def)
+  apply (erule conjE)
+  using cast_lemma2 
+  by metis
+
+
+lemma subl_subgoal_ri:
+      "bins = BPF_ALU BPF_SUB dst (SOImm src) \<Longrightarrow>
+       xins = Psubl_ri rd imm \<Longrightarrow>
+       (BPF_OK pc rs' m' ss' is_v1 (cur_cu+1) remain_cu) = step fuel bins rs m ss is_v1 cur_cu remain_cu \<Longrightarrow>
+       Next reg' m'  = exec_instr xins sz reg m \<Longrightarrow> 
+       rd = bpf_to_x64_reg dst \<Longrightarrow>
+       imm = ucast (src) \<Longrightarrow>
+       reg (IR rd) = Vint n1 \<Longrightarrow>
+       ucast n1  = rs dst \<Longrightarrow>
+       reg' (IR rd) = Vint n3 \<Longrightarrow>
+       ucast n3 = rs'dst"
+  apply (unfold exec_instr_def step)
+  apply simp
+  apply (unfold eval_alu32_def)
+  apply (cases BPF_SUB, simp_all)
+  apply (unfold eval_alu32_aux1_def)
+  apply (unfold Let_def)
+  apply (cases BPF_SUB, simp_all)
+  apply (unfold sub32_def )
+  apply (unfold nextinstr_nf_def nextinstr_def eval_reg_def)
+  apply simp
+  apply (unfold add64_def)
+  apply (erule conjE)
+  apply (cases "is_v1", simp_all)
+  apply (cases "is_v1", simp_all)
+  using cast_lemma2 
+
+qed
+
+
+
+(*
+lemma addq_subgoal_rr:
+      "bins = BPF_ALU64 BPF_ADD dst (SOReg src) \<Longrightarrow>
+       xins = Paddq_rr rd ri \<Longrightarrow>
+       (BPF_OK pc rs' m' ss' is_v1 (cur_cu+1) remain_cu) = step fuel bins rs m ss is_v1 cur_cu remain_cu \<Longrightarrow>
+       Next reg' m' = exec_instr xins sz reg m \<Longrightarrow> 
+       rd = bpf_to_x64_reg dst \<Longrightarrow>
+       ri = bpf_to_x64_reg src \<Longrightarrow>
+       reg (IR rd) = Vlong n1 \<Longrightarrow>
+       reg (IR ri) = Vlong n2 \<Longrightarrow>
+       n1  = rs dst \<Longrightarrow>
+       n2  = rs src \<Longrightarrow>
+       Vlong (rs' dst) = reg' (IR (bpf_to_x64_reg dst))"
+  apply (unfold exec_instr_def step,simp_all)
+  apply (unfold eval_alu64_def)
+  apply (cases BPF_ADD, simp_all)
+  apply (unfold add64_def eval_alu64_aux1_def Let_def)
+  apply (cases BPF_ADD)
+  apply (unfold nextinstr_nf_def nextinstr_def eval_reg_def)
+  by simp_all
+
+lemma addq_subgoal_rr_aux2_1:"xins = Paddq_rr dst src \<Longrightarrow> Next reg' m' = exec_instr xins sz reg m \<Longrightarrow> \<forall> r \<noteq> dst . reg' (IR r) = reg (IR r)"
+  apply(unfold exec_instr_def, cases "xins", simp_all)
+  apply(unfold nextinstr_nf_def nextinstr_def add64_def) 
+  by auto
+
+lemma addq_subgoal_rr_aux2_2:"xins = Paddq_rr (bpf_to_x64_reg dst) (bpf_to_x64_reg src) \<Longrightarrow> Next reg' m' = exec_instr xins sz reg m \<Longrightarrow>
+       \<forall> r \<noteq> bpf_to_x64_reg dst. reg' (IR r) = reg (IR r)"
+  using addq_subgoal_rr_aux2_1 by blast
+
+lemma addq_subgoal_rr_aux2:"xins = Paddq_rr (bpf_to_x64_reg dst) (bpf_to_x64_reg src) \<Longrightarrow> Next reg' m' = exec_instr xins sz reg m \<Longrightarrow>
+       \<forall> r \<noteq> dst. reg' (IR (bpf_to_x64_reg r)) = reg (IR (bpf_to_x64_reg r))"
+  using bpf_to_x64_reg_corr addq_subgoal_rr_aux2_2 by metis
+
+lemma addq_subgoal_rr_aux3:"bins = BPF_ALU64 BPF_ADD dst (SOReg src) \<Longrightarrow> (BPF_OK pc rs' m' ss' is_v1 (cur_cu+1) remain_cu) = step fuel bins rs m ss is_v1 cur_cu remain_cu \<Longrightarrow>
+       \<forall> r \<noteq> dst. rs' r = rs r"
+  apply(cases "bins",simp_all)
+  apply(unfold eval_alu64_def,simp)
+  by (unfold eval_alu64_aux1_def, simp)
+
+*)
+
+(*
+lemma subq_subgoal_rr_aux1:
+     "bins = BPF_ALU64 BPF_SUB dst (SOReg src) \<Longrightarrow>
+     xins = Psubq_rr rd ri \<Longrightarrow>
+     (BPF_OK pc rs' m' ss' is_v1 (cur_cu+1) remain_cu) = step fuel bins rs m ss is_v1 cur_cu remain_cu \<Longrightarrow>
+     Next reg' m' = exec_instr xins sz reg m \<Longrightarrow>
+     rd = (bpf_to_x64_reg dst) \<Longrightarrow>
+     ri = (bpf_to_x64_reg src) \<Longrightarrow>
+     reg (IR rd) = Vlong n1 \<Longrightarrow>
+     reg (IR ri) = Vlong n2 \<Longrightarrow>
+     n1  = rs dst \<Longrightarrow>
+     n2  = rs src \<Longrightarrow> 
+     Vlong (rs' dst) = reg' (IR (bpf_to_x64_reg dst))"
+  apply (unfold exec_instr_def step)
+  apply simp
+  apply (unfold eval_alu64_def)
+  apply (cases BPF_SUB, simp_all)
+  apply (unfold eval_alu64_aux1_def)
+  apply (unfold Let_def)
+  apply (cases BPF_SUB, simp_all)
+  apply (unfold sub64_def)
+  apply (unfold nextinstr_nf_def nextinstr_def eval_reg_def)
+  by simp
+
+lemma subq_subgoal_rr_aux2_1:"xins = Psubq_rr dst src \<Longrightarrow> Next reg' m' = exec_instr xins sz reg m \<Longrightarrow> \<forall> r \<noteq> dst . reg' (IR r) = reg (IR r)"
+  apply(unfold exec_instr_def, cases "xins", simp_all)
+  apply(unfold nextinstr_nf_def nextinstr_def add64_def) 
+  by auto
+
+lemma subq_subgoal_rr_aux2_2:"xins = Psubq_rr (bpf_to_x64_reg dst) (bpf_to_x64_reg src) \<Longrightarrow> Next reg' m' = exec_instr xins sz reg m \<Longrightarrow>
+       \<forall> r \<noteq> bpf_to_x64_reg dst. reg' (IR r) = reg (IR r)"
+  using subq_subgoal_rr_aux2_1 by blast
+
+lemma subq_subgoal_rr_aux2:"xins = Psubq_rr (bpf_to_x64_reg dst) (bpf_to_x64_reg src) \<Longrightarrow> Next reg' m' = exec_instr xins sz reg m \<Longrightarrow>
+       \<forall> r \<noteq> dst. reg' (IR (bpf_to_x64_reg r)) = reg (IR (bpf_to_x64_reg r))"
+  using bpf_to_x64_reg_corr subq_subgoal_rr_aux2_2 by metis
+
+
+lemma subq_subgoal_rr_aux3:"bins = BPF_ALU64 BPF_SUB dst (SOReg src) \<Longrightarrow> (BPF_OK pc rs' m' ss' is_v1 (cur_cu+1) remain_cu) = step fuel bins rs m ss is_v1 cur_cu remain_cu \<Longrightarrow>
+       \<forall> r \<noteq> dst. rs' r = rs r"
+  apply(cases "bins",simp_all)
+  apply(unfold eval_alu64_def,simp)
+  by (unfold eval_alu64_aux1_def, simp)
+*)
+
+(*lemma interp2_aux1:
+  assumes a0:"length xins = (2::nat)" and 
+          a1:"result = interp2 n xins (Next reg m)"
+        shows "result = Next reg' m' \<longrightarrow> n\<ge>2"
+proof (rule ccontr)
+  assume a2:"\<not> (result = Next reg' m' \<longrightarrow> n\<ge>2)"
+  let ?res_ok = "Next reg' m'"
+  have a3:"\<not> (\<not> result = ?res_ok \<or> (n\<ge>2))" using imp_conv_disj a2 by blast
+  have a4:"result = ?res_ok \<and> n<2" using a3 by simp
+   then show "False"
+   proof
+     have b0:"n<2" using a4 conjE by simp
+     have b2: "interp2 n xins (Next reg m) = Stuck"using a0 exec_instr_def 
+       by (smt (verit, del_insts) b0 interp2.elims interp2.simps(2) length_0_conv less_2_cases nat.inject outcome.simps(4) zero_neq_numeral)
+     thus "False" using b2 
+       using a1 a4 by (simp add: a0 exec_instr_def)
+   qed
+ qed
+
+lemma interp2_aux2:
+  assumes a0:"length xins = (2::nat)" and 
+          a1:"result = interp2 n xins (Next reg m)"
+        shows "result = Next reg' m' \<longrightarrow> (exec_instr (xins!0) 1 reg m) \<noteq> Stuck"
+proof (rule ccontr)
+  assume a2:"\<not> (result = Next reg' m' \<longrightarrow> (exec_instr (xins!0) 1 reg m) \<noteq> Stuck)"
+  let ?tmp = "(exec_instr (xins!0) 1 reg m) "
+  let ?res_ok = "Next reg' m'"
+  have a3:"\<not> (\<not> result = ?res_ok \<or> ?tmp \<noteq> Stuck)" using imp_conv_disj a2 by blast
+  have a4:"result = ?res_ok \<and> ?tmp = Stuck" using a3 by simp
+   then show "False"
+   proof
+     have b0:"?tmp = Stuck" using a4 conjE by simp
+     have b1:"xins\<noteq>[]" using a0 by auto
+     have b2: "interp2 n xins (Next reg m) = Stuck"using a0 b0 b1 exec_instr_def 
+       by (smt (verit, del_insts) interp2.elims nth_Cons_0 outcome.case(2) outcome.simps(4))
+     thus "False" using b2 
+       using a1 a4 by (simp add: a0 exec_instr_def)
+   qed
+ qed
+
+(*interp2 n (drop 1 xins) (Next reg' m') = (exec_instr (xins!1) 1 reg' m')*)
+lemma interp2_aux3:
+  assumes a0:"length xins = (2::nat)" and 
+          a1:"result = interp2 n xins (Next reg m)" and
+          a2:"Next reg' m' = (exec_instr (xins!0) 1 reg m)"
+        shows "result = Next reg'' m'' \<longrightarrow> (exec_instr (xins!1) 1 reg' m') \<noteq> Stuck"
+proof (rule ccontr)
+  assume a2:"\<not> (result = Next reg'' m'' \<longrightarrow> (exec_instr (xins!1) 1 reg' m') \<noteq> Stuck)"
+  let ?tmp = "(exec_instr (xins!1) 1 reg' m') "
+  let ?res_ok = "Next reg'' m''"
+  have a3:"\<not> (\<not> result = ?res_ok \<or> ?tmp \<noteq> Stuck)" using imp_conv_disj a2 by blast
+  have a4:"result = ?res_ok \<and> ?tmp = Stuck" using a3 by simp
+   then show "False"
+   proof
+     have b0:"?tmp = Stuck" using a4 conjE by simp
+     have b1:"xins\<noteq>[]" using a0 by auto
+     have b2:"interp2 (n-1) (drop 1 xins) (Next reg' m') = (exec_instr (xins!1) 1 reg' m')" using a0 a1 a2 b1 
+       by (smt (verit, ccfv_threshold) Cons_nth_drop_Suc One_nat_def Suc_n_not_le_n drop_eq_Nil interp2.elims lessI list.inject numeral_2_eq_2 outcome.case(2) outcome.simps(4))
+     have b3: "interp2 (n-1) (drop 1 xins) (Next reg' m') = Stuck"using a0 b0 b1 exec_instr_def a2
+       using interp2.elims nth_Cons_0 outcome.case(2) outcome.simps(4) using b2 by simp
+     have b4: "interp2 n xins (Next reg m) = Stuck" using a0 a1 b3 exec_instr_def a2 b1
+       by (smt (verit) Cons_nth_drop_Suc One_nat_def Suc_n_not_le_n assms(3) drop0 drop_eq_Nil interp2.elims list.inject list_consists_2 numeral_2_eq_2 outcome.case(2) outcome.simps(4) zero_less_Suc)
+     thus "False" using b2 
+       using a1 a4 by (simp add: a0 exec_instr_def)
+   qed
+ qed
+
+
+lemma interp2_aux4:"n > 0 \<Longrightarrow> interp2 n [] (Next reg m) = Next reg m"
+  by (metis Suc_pred interp2.simps(2))
+
+
+lemma interp2_aux4: assumes a0:"Next reg2 m2 = interp2 n xins (Next reg m)" and
+  a1:"length xins = (2::nat)"
+shows" \<exists> reg' m'. Next reg' m' = (exec_instr (xins!0) 1 reg m) \<and> Next reg2 m2 = (exec_instr (xins!1) 1 reg' m')  "
+proof-
+  have b0:"n\<ge>2" using a0 a1 interp2_aux1 by blast
+  from a0 a1 have "\<exists> result1. result1 = (exec_instr (xins!0) 1 reg m)" by simp
+  then obtain result1 where " result1 = (exec_instr (xins!0) 1 reg m)" by simp
+  have b1:"result1 \<noteq> Stuck" using interp2_aux2 a0 a1 
+    by (metis \<open>(result1::outcome) = exec_instr ((xins::instruction list) ! (0::nat)) (1::64 word) (reg::preg \<Rightarrow> val) (m::64 word \<Rightarrow> 8 word option option)\<close> a0 a1)
+  from b1 have "\<exists> reg' m'. Next reg' m' = result1" 
+    by (metis outcome.exhaust)
+  then obtain reg' m' where "Next reg' m' = result1" by blast
+  have "\<exists> result2. result2 = (exec_instr (xins!1) 1 reg' m')" by simp
+  then obtain result2 where " result2 = (exec_instr (xins!1) 1 reg' m')" by simp
+  have b3:"result2 \<noteq> Stuck" using interp2_aux3 a0 a1 
+    by (metis \<open>(result1::outcome) = exec_instr ((xins::instruction list) ! (0::nat)) (1::64 word) (reg::preg \<Rightarrow> val) (m::64 word \<Rightarrow> 8 word option option)\<close> \<open>(result2::outcome) = exec_instr ((xins::instruction list) ! (1::nat)) (1::64 word) (reg'::preg \<Rightarrow> val) (m'::64 word \<Rightarrow> 8 word option option)\<close> \<open>Next (reg'::preg \<Rightarrow> val) (m'::64 word \<Rightarrow> 8 word option option) = (result1::outcome)\<close>)
+  then obtain reg'' m'' where "Next reg'' m'' = result2" 
+    by (metis outcome.exhaust)
+  have b4:"Next reg'' m'' = Next reg2 m2" using b1 interp2_aux4 interp2_aux1 try
+  show ?thesis using a0 a1 b0 
+    using \<open>(result1::outcome) = exec_instr ((xins::instruction list) ! (0::nat)) (1::64 word) (reg::preg \<Rightarrow> val) (m::64 word \<Rightarrow> 8 word option option)\<close> \<open>(result2::outcome) = exec_instr ((xins::instruction list) ! (1::nat)) (1::64 word) (reg'::preg \<Rightarrow> val) (m'::64 word \<Rightarrow> 8 word option option)\<close> \<open>Next (reg''::preg \<Rightarrow> val) (m''::64 word \<Rightarrow> 8 word option option) = (result2::outcome)\<close> \<open>Next (reg'::preg \<Rightarrow> val) (m'::64 word \<Rightarrow> 8 word option option) = (result1::outcome)\<close> b4 by blast
+qed
+lemma shift_subgoal_rr_aux1_1:"Next reg'' m'' = interp2 n xins (Next reg m) \<Longrightarrow> length xins = (2::nat) \<Longrightarrow> \<exists> reg' m'. Next reg' m' = (exec_instr (xins!0) 1 reg m) \<and> Next reg'' m'' = (exec_instr (xins!1) 1 reg' m')  "
+  using interp2_aux4 by simp
+
+
+lemma shift_subgoal_rr_aux1_2:
+  assumes a0:"length xins = (2::nat)" and a1:"Next reg' m' = (exec_instr (xins!0) 1 reg m)" and a1:" Next reg'' m'' = (exec_instr (xins!1) 1 reg' m')"
+  shows "Next reg'' m'' = interp2 n xins (Next reg m)"
+  sorry
+
+lemma shift_subgoal_rr_aux2:
+  assumes a0:"xins = [(Pmovq_rr src (x64Syntax.RCX)),(Pshlq_r dst)]" and 
+    a1:"Next reg'' m'' = interp2 n xins (Next reg m) " 
+  shows " m'' = m"
+proof-
+  have b0:"length xins = (2::nat)" using a0 by simp
+  thus ?thesis using b0 a0 a1 shift_subgoal_rr_aux2_3 
+    by (meson shift_subgoal_rr_aux1_1)
+qed
+
+
+lemma push_pop_subgoal_rr_aux2_2:
+  assumes a0:"xins = [Ppushl_r x64Syntax.RCX, Ppopl x64Syntax.RCX]" and 
+    a1:"Next reg'' m'' = interp2 n xins (Next reg m)" and
+    a2:"storev M32 m (sub64 (reg (IR SP)) (vlong_of_memory_chunk M32)) (reg (IR ireg.RCX)) \<noteq> None "
+  shows "reg'' (IR x64Syntax.RCX) = reg (IR x64Syntax.RCX)"
+proof-
+  have b0:"length xins = (2::nat)" using a0 by simp
+  thus ?thesis using b0 a0 a1 a2 push_pop_subgoal_rr_aux2_1 shift_subgoal_rr_aux1_1
+    by metis
+qed
+*)
+
+
+end
